cluster/isabelle/Zen.thy
@@ -315,19 +315,21 @@ locale zen = zenMessages +
     "\<And>n. currentVotingNodes (nodeState n) = V (firstUncommittedSlot (nodeState n))"
   assumes firstUncommittedSlot_PublishRequest:
     "\<And>i n t x. firstUncommittedSlot (nodeState n) < i \<Longrightarrow> \<not> n \<midarrow>\<langle> PublishRequest i t x \<rangle>\<leadsto>"
-  assumes firstUncommittedSlot_PublishResponse:
-    "\<And>i n t. firstUncommittedSlot (nodeState n) < i \<Longrightarrow> \<not> n \<midarrow>\<langle> PublishResponse i t \<rangle>\<leadsto>"
+  assumes lastAcceptedSlot_firstUncommittedSlot:
+    "\<And>n. lastAcceptedSlot (nodeState n) \<le> firstUncommittedSlot (nodeState n)"
+  assumes lastAcceptedSlot_PublishResponse:
+    "\<And>i n t. lastAcceptedSlot (nodeState n) < i \<Longrightarrow> \<not> n \<midarrow>\<langle> PublishResponse i t \<rangle>\<leadsto>"
   assumes lastAcceptedTerm_None: "\<And>n t. lastAcceptedTerm (nodeState n) = None
-    \<Longrightarrow> \<not> n \<midarrow>\<langle> PublishResponse (firstUncommittedSlot (nodeState n)) t \<rangle>\<leadsto>"
+    \<Longrightarrow> \<not> n \<midarrow>\<langle> PublishResponse (lastAcceptedSlot (nodeState n)) t \<rangle>\<leadsto>"
   assumes lastAcceptedTerm_Some_sent: "\<And>n t. lastAcceptedTerm (nodeState n) = Some t
-    \<Longrightarrow> n \<midarrow>\<langle> PublishResponse (firstUncommittedSlot (nodeState n)) t \<rangle>\<leadsto>"
+    \<Longrightarrow> n \<midarrow>\<langle> PublishResponse (lastAcceptedSlot (nodeState n)) t \<rangle>\<leadsto>"
   assumes lastAcceptedTerm_Some_max: "\<And>n t t'. lastAcceptedTerm (nodeState n) = Some t
-    \<Longrightarrow> n \<midarrow>\<langle> PublishResponse (firstUncommittedSlot (nodeState n)) t' \<rangle>\<leadsto>
+    \<Longrightarrow> n \<midarrow>\<langle> PublishResponse (lastAcceptedSlot (nodeState n)) t' \<rangle>\<leadsto>
     \<Longrightarrow> t' \<le> t"
   assumes lastAcceptedTerm_Some_currentTerm: "\<And>n t. lastAcceptedTerm (nodeState n) = Some t
     \<Longrightarrow> t \<le> currentTerm (nodeState n)"
   assumes lastAcceptedTerm_Some_value: "\<And>n t. lastAcceptedTerm (nodeState n) = Some t
-    \<Longrightarrow> \<langle> PublishRequest (firstUncommittedSlot (nodeState n)) t (lastAcceptedValue (nodeState n)) \<rangle>\<leadsto>"
+    \<Longrightarrow> \<langle> PublishRequest (lastAcceptedSlot (nodeState n)) t (lastAcceptedValue (nodeState n)) \<rangle>\<leadsto>"
   assumes JoinRequest_currentTerm:
     "\<And>n i t a. n \<midarrow>\<langle> JoinRequest i t a \<rangle>\<leadsto> \<Longrightarrow> t \<le> currentTerm (nodeState n)"
   assumes JoinRequest_slot_function:
@@ -357,7 +359,7 @@ locale zen = zenMessages +
     \<Longrightarrow> \<exists> n' \<in> joinVotes (nodeState n).
          (n' \<midarrow>\<langle> JoinRequest (firstUncommittedSlot (nodeState n))
                                (currentTerm (nodeState n))
-                               (lastAcceptedTerm (nodeState n)) \<rangle>\<rightarrow> (OneNode n))"
+                               (lastAcceptedTermInSlot (nodeState n)) \<rangle>\<rightarrow> (OneNode n))"
   assumes electionValueForced_max: "\<And>n n' a'.
     \<lbrakk> electionValueForced (nodeState n);
       \<not> (\<exists> x. \<langle> PublishRequest (firstUncommittedSlot (nodeState n)) (currentTerm (nodeState n)) x \<rangle>\<leadsto>);
@@ -365,7 +367,7 @@ locale zen = zenMessages +
       n' \<midarrow>\<langle> JoinRequest (firstUncommittedSlot (nodeState n))
                                 (currentTerm (nodeState n))
                                 a' \<rangle>\<rightarrow> (OneNode n) \<rbrakk>
-    \<Longrightarrow> maxTermOption a' (lastAcceptedTerm (nodeState n)) = lastAcceptedTerm (nodeState n)"
+    \<Longrightarrow> maxTermOption a' (lastAcceptedTermInSlot (nodeState n)) = lastAcceptedTermInSlot (nodeState n)"
   assumes publishVotes: "\<And>n n'. n' \<in> publishVotes (nodeState n)
     \<Longrightarrow> n' \<midarrow>\<langle> PublishResponse (firstUncommittedSlot (nodeState n)) (currentTerm (nodeState n)) \<rangle>\<leadsto>"
   assumes publishVotes_currentVotingNodes: "\<And>n. publishVotes (nodeState n) \<subseteq> currentVotingNodes (nodeState n)"
@@ -460,11 +462,12 @@ lemma (in zenStep)
   assumes "\<And>n. committed\<^sub><' (firstUncommittedSlot (nodeState' n))"
   assumes "\<And>n. currentVotingNodes (nodeState' n) = V' (firstUncommittedSlot (nodeState' n))"
   assumes "\<And>i n t x. firstUncommittedSlot (nodeState' n) < i \<Longrightarrow> \<not> n \<midarrow>\<langle> PublishRequest i t x \<rangle>\<leadsto>'"
-  assumes "\<And>i n t. firstUncommittedSlot (nodeState' n) < i \<Longrightarrow> \<not> n \<midarrow>\<langle> PublishResponse i t \<rangle>\<leadsto>'"
-  assumes "\<And>n t. lastAcceptedTerm (nodeState' n) = None \<Longrightarrow> \<not> n \<midarrow>\<langle> PublishResponse (firstUncommittedSlot (nodeState' n)) t \<rangle>\<leadsto>'"
-  assumes "\<And>n t. lastAcceptedTerm (nodeState' n) = Some t \<Longrightarrow> n \<midarrow>\<langle> PublishResponse (firstUncommittedSlot (nodeState' n)) t \<rangle>\<leadsto>'"
-  assumes "\<And>n t t'. lastAcceptedTerm (nodeState' n) = Some t \<Longrightarrow> n \<midarrow>\<langle> PublishResponse (firstUncommittedSlot (nodeState' n)) t' \<rangle>\<leadsto>' \<Longrightarrow> t' \<le> t"
-  assumes "\<And>n t. lastAcceptedTerm (nodeState' n) = Some t \<Longrightarrow> \<langle> PublishRequest (firstUncommittedSlot (nodeState' n)) t (lastAcceptedValue (nodeState' n)) \<rangle>\<leadsto>'"
+  assumes "\<And>n. lastAcceptedSlot (nodeState' n) \<le> firstUncommittedSlot (nodeState' n)"
+  assumes "\<And>i n t. lastAcceptedSlot (nodeState' n) < i \<Longrightarrow> \<not> n \<midarrow>\<langle> PublishResponse i t \<rangle>\<leadsto>'"
+  assumes "\<And>n t. lastAcceptedTerm (nodeState' n) = None \<Longrightarrow> \<not> n \<midarrow>\<langle> PublishResponse (lastAcceptedSlot (nodeState' n)) t \<rangle>\<leadsto>'"
+  assumes "\<And>n t. lastAcceptedTerm (nodeState' n) = Some t \<Longrightarrow> n \<midarrow>\<langle> PublishResponse (lastAcceptedSlot (nodeState' n)) t \<rangle>\<leadsto>'"
+  assumes "\<And>n t t'. lastAcceptedTerm (nodeState' n) = Some t \<Longrightarrow> n \<midarrow>\<langle> PublishResponse (lastAcceptedSlot (nodeState' n)) t' \<rangle>\<leadsto>' \<Longrightarrow> t' \<le> t"
+  assumes "\<And>n t. lastAcceptedTerm (nodeState' n) = Some t \<Longrightarrow> \<langle> PublishRequest (lastAcceptedSlot (nodeState' n)) t (lastAcceptedValue (nodeState' n)) \<rangle>\<leadsto>'"
   assumes "\<And>n t. lastAcceptedTerm (nodeState' n) = Some t \<Longrightarrow> t \<le> currentTerm (nodeState' n)"
   assumes "\<And>n i t a. n \<midarrow>\<langle> JoinRequest i t a \<rangle>\<leadsto>' \<Longrightarrow> t \<le> currentTerm (nodeState' n)"
   assumes "\<And>n i i' t a a'. n \<midarrow>\<langle> JoinRequest i t a \<rangle>\<leadsto>' \<Longrightarrow> n \<midarrow>\<langle> JoinRequest i' t a' \<rangle>\<leadsto>' \<Longrightarrow> i = i'"
@@ -473,8 +476,8 @@ lemma (in zenStep)
   assumes "\<And>n n'. n' \<in> joinVotes (nodeState' n) \<Longrightarrow> promised' (firstUncommittedSlot (nodeState' n)) n' n (currentTerm (nodeState' n))"
   assumes "\<And>n. electionWon (nodeState' n) \<Longrightarrow> isQuorum (nodeState' n) (joinVotes (nodeState' n))"
   assumes "\<And>n n'. \<not> electionValueForced (nodeState' n) \<Longrightarrow> n' \<in> joinVotes (nodeState' n) \<Longrightarrow> n' \<midarrow>\<langle> JoinRequest (firstUncommittedSlot (nodeState' n)) (currentTerm (nodeState' n)) None \<rangle>\<rightarrow>' (OneNode n) \<or> (\<exists>i<firstUncommittedSlot (nodeState' n). \<exists>a. n' \<midarrow>\<langle> JoinRequest i (currentTerm (nodeState' n)) a \<rangle>\<rightarrow>' (OneNode n))"
-  assumes "\<And>n. electionValueForced (nodeState' n) \<Longrightarrow> \<not> (\<exists>x. \<langle> PublishRequest (firstUncommittedSlot (nodeState' n)) (currentTerm (nodeState' n)) x \<rangle>\<leadsto>') \<Longrightarrow> \<exists>n'\<in>joinVotes (nodeState' n). n' \<midarrow>\<langle> JoinRequest (firstUncommittedSlot (nodeState' n)) (currentTerm (nodeState' n)) (lastAcceptedTerm (nodeState' n)) \<rangle>\<rightarrow>' (OneNode n)"
-  assumes "\<And>n n' a'. electionValueForced (nodeState' n) \<Longrightarrow> \<not> (\<exists>x. \<langle> PublishRequest (firstUncommittedSlot (nodeState' n)) (currentTerm (nodeState' n)) x \<rangle>\<leadsto>') \<Longrightarrow> n' \<in> joinVotes (nodeState' n) \<Longrightarrow> n' \<midarrow>\<langle> JoinRequest (firstUncommittedSlot (nodeState' n)) (currentTerm (nodeState' n)) a' \<rangle>\<rightarrow>' (OneNode n) \<Longrightarrow> maxTermOption a' (lastAcceptedTerm (nodeState' n)) = lastAcceptedTerm (nodeState' n)"
+  assumes "\<And>n. electionValueForced (nodeState' n) \<Longrightarrow> \<not> (\<exists>x. \<langle> PublishRequest (firstUncommittedSlot (nodeState' n)) (currentTerm (nodeState' n)) x \<rangle>\<leadsto>') \<Longrightarrow> \<exists>n'\<in>joinVotes (nodeState' n). n' \<midarrow>\<langle> JoinRequest (firstUncommittedSlot (nodeState' n)) (currentTerm (nodeState' n)) (lastAcceptedTermInSlot (nodeState' n)) \<rangle>\<rightarrow>' (OneNode n)"
+  assumes "\<And>n n' a'. electionValueForced (nodeState' n) \<Longrightarrow> \<not> (\<exists>x. \<langle> PublishRequest (firstUncommittedSlot (nodeState' n)) (currentTerm (nodeState' n)) x \<rangle>\<leadsto>') \<Longrightarrow> n' \<in> joinVotes (nodeState' n) \<Longrightarrow> n' \<midarrow>\<langle> JoinRequest (firstUncommittedSlot (nodeState' n)) (currentTerm (nodeState' n)) a' \<rangle>\<rightarrow>' (OneNode n) \<Longrightarrow> maxTermOption a' (lastAcceptedTermInSlot (nodeState' n)) = lastAcceptedTermInSlot (nodeState' n)"
   assumes "\<And>n n'. n' \<in> publishVotes (nodeState' n) \<Longrightarrow> n' \<midarrow>\<langle> PublishResponse (firstUncommittedSlot (nodeState' n)) (currentTerm (nodeState' n)) \<rangle>\<leadsto>'"
   assumes "\<And>n. publishVotes (nodeState' n) \<subseteq> currentVotingNodes (nodeState' n)"
   assumes "\<And>n. currentClusterState (nodeState' n) = lastCommittedClusterStateBefore' (firstUncommittedSlot (nodeState' n))"
@@ -483,18 +486,18 @@ lemma (in zenStep)
   assumes "\<And>i conf cs. \<langle> CatchUpResponse i conf cs \<rangle>\<leadsto>' \<Longrightarrow> lastCommittedClusterStateBefore' i = cs"
   shows zenI: "zen messages' nodeState'"
   apply (unfold_locales)
-                 apply (fold isMessageFromTo'_def)
-                 apply (fold isMessageTo'_def)
-                 apply (fold isMessageFrom'_def)
-                 apply (fold isMessage'_def)
-                 apply (fold v'_def)
-                 apply (fold isCommitted'_def)
-                 apply (fold committedTo'_def)
-                 apply (fold v\<^sub>c'_def)
-                 apply (fold V'_def)
-                 apply (fold promised'_def)
-                 apply (fold prevAccepted'_def)
-                 apply (fold lastCommittedClusterStateBefore'_def)
+                      apply (fold isMessageFromTo'_def)
+                      apply (fold isMessageTo'_def)
+                      apply (fold isMessageFrom'_def)
+                      apply (fold isMessage'_def)
+                      apply (fold v'_def)
+                      apply (fold isCommitted'_def)
+                      apply (fold committedTo'_def)
+                      apply (fold v\<^sub>c'_def)
+                      apply (fold V'_def)
+                      apply (fold promised'_def)
+                      apply (fold prevAccepted'_def)
+                      apply (fold lastCommittedClusterStateBefore'_def)
   using assms proof - qed
 
 lemma (in zenStep)
@@ -554,6 +557,8 @@ proof -
     "\<And>n. electionValueForced (nodeState' n) = electionValueForced (nodeState n)"
     "\<And>n. lastAcceptedTerm (nodeState' n) = lastAcceptedTerm (nodeState n)"
     "\<And>n. lastAcceptedValue (nodeState' n) = lastAcceptedValue (nodeState n)"
+    "\<And>n. lastAcceptedSlot (nodeState' n) = lastAcceptedSlot (nodeState n)"
+    "\<And>n. lastAcceptedTermInSlot (nodeState' n) = lastAcceptedTermInSlot (nodeState n)"
     by (unfold nodeState', auto)
 
   have v_eq[simp]: "v' = v" by (intro ext, auto simp add: v'_def v_def message_simps)
@@ -581,16 +586,17 @@ proof -
     from JoinRequest_unique_destination show "\<And>i' i s t a a' d d'. s \<midarrow>\<langle> JoinRequest i t a \<rangle>\<rightarrow> d \<Longrightarrow> s \<midarrow>\<langle> JoinRequest i' t a' \<rangle>\<rightarrow> d' \<Longrightarrow> d = d'".
     from currentNode_nodeState show "\<And>n. currentNode (nodeState n) = n" .
     from committedTo_firstUncommittedSlot show "\<And>n. committed\<^sub>< (firstUncommittedSlot (nodeState n))" .
-    from firstUncommittedSlot_PublishResponse show "\<And>n i t. firstUncommittedSlot (nodeState n) < i \<Longrightarrow> \<not> n \<midarrow>\<langle> PublishResponse i t \<rangle>\<leadsto>" .
-    from lastAcceptedTerm_None show "\<And>n t. lastAcceptedTerm (nodeState n) = None \<Longrightarrow> \<not> n \<midarrow>\<langle> PublishResponse (firstUncommittedSlot (nodeState n)) t \<rangle>\<leadsto>".
-    from lastAcceptedTerm_Some_sent show "\<And>n t. lastAcceptedTerm (nodeState n) = Some t \<Longrightarrow> n \<midarrow>\<langle> PublishResponse (firstUncommittedSlot (nodeState n)) t \<rangle>\<leadsto>".
-    from lastAcceptedTerm_Some_max show "\<And>n t t'. lastAcceptedTerm (nodeState n) = Some t \<Longrightarrow> n \<midarrow>\<langle> PublishResponse (firstUncommittedSlot (nodeState n)) t' \<rangle>\<leadsto> \<Longrightarrow> t' \<le> t".
+    from lastAcceptedSlot_firstUncommittedSlot  show "\<And>n. lastAcceptedSlot (nodeState n) \<le> firstUncommittedSlot (nodeState n)".
+    from lastAcceptedSlot_PublishResponse show "\<And>n i t. lastAcceptedSlot (nodeState n) < i \<Longrightarrow> \<not> n \<midarrow>\<langle> PublishResponse i t \<rangle>\<leadsto>" .
+    from lastAcceptedTerm_None show "\<And>n t. lastAcceptedTerm (nodeState n) = None \<Longrightarrow> \<not> n \<midarrow>\<langle> PublishResponse (lastAcceptedSlot (nodeState n)) t \<rangle>\<leadsto>".
+    from lastAcceptedTerm_Some_sent show "\<And>n t. lastAcceptedTerm (nodeState n) = Some t \<Longrightarrow> n \<midarrow>\<langle> PublishResponse (lastAcceptedSlot (nodeState n)) t \<rangle>\<leadsto>".
+    from lastAcceptedTerm_Some_max show "\<And>n t t'. lastAcceptedTerm (nodeState n) = Some t \<Longrightarrow> n \<midarrow>\<langle> PublishResponse (lastAcceptedSlot (nodeState n)) t' \<rangle>\<leadsto> \<Longrightarrow> t' \<le> t".
     from JoinRequest_currentTerm show "\<And>n i t a. n \<midarrow>\<langle> JoinRequest i t a \<rangle>\<leadsto> \<Longrightarrow> t \<le> currentTerm (nodeState n)".
     from JoinRequest_slot_function show "\<And>n i i' t a a'. n \<midarrow>\<langle> JoinRequest i t a \<rangle>\<leadsto> \<Longrightarrow> n \<midarrow>\<langle> JoinRequest i' t a' \<rangle>\<leadsto> \<Longrightarrow> i = i'".
     from electionWon_isQuorum show "\<And>n. electionWon (nodeState n) \<Longrightarrow> isQuorum (nodeState n) (joinVotes (nodeState n))".
     from electionValueFree_JoinRequest show "\<And>n n'. \<not> electionValueForced (nodeState n) \<Longrightarrow> n' \<in> joinVotes (nodeState n) \<Longrightarrow> n' \<midarrow>\<langle> JoinRequest (firstUncommittedSlot (nodeState n)) (currentTerm (nodeState n)) None \<rangle>\<rightarrow> (OneNode n) \<or> (\<exists>i<firstUncommittedSlot (nodeState n). \<exists>a. n' \<midarrow>\<langle> JoinRequest i (currentTerm (nodeState n)) a \<rangle>\<rightarrow> (OneNode n))".
-    from electionValueForced_JoinRequest show "\<And>n. electionValueForced (nodeState n) \<Longrightarrow> \<not> (\<exists>x. \<langle> PublishRequest (firstUncommittedSlot (nodeState n)) (currentTerm (nodeState n)) x \<rangle>\<leadsto>) \<Longrightarrow> \<exists>n'\<in>joinVotes (nodeState n). n' \<midarrow>\<langle> JoinRequest (firstUncommittedSlot (nodeState n)) (currentTerm (nodeState n)) (lastAcceptedTerm (nodeState n)) \<rangle>\<rightarrow> (OneNode n)".
-    from electionValueForced_max show " \<And>n n' a'. electionValueForced (nodeState n) \<Longrightarrow> \<not> (\<exists>x. \<langle> PublishRequest (firstUncommittedSlot (nodeState n)) (currentTerm (nodeState n)) x \<rangle>\<leadsto>) \<Longrightarrow> n' \<in> joinVotes (nodeState n) \<Longrightarrow> n' \<midarrow>\<langle> JoinRequest (firstUncommittedSlot (nodeState n)) (currentTerm (nodeState n)) a' \<rangle>\<rightarrow> (OneNode n) \<Longrightarrow> maxTermOption a' (lastAcceptedTerm (nodeState n)) = lastAcceptedTerm (nodeState n)".
+    from electionValueForced_JoinRequest show "\<And>n. electionValueForced (nodeState n) \<Longrightarrow> \<not> (\<exists>x. \<langle> PublishRequest (firstUncommittedSlot (nodeState n)) (currentTerm (nodeState n)) x \<rangle>\<leadsto>) \<Longrightarrow> \<exists>n'\<in>joinVotes (nodeState n). n' \<midarrow>\<langle> JoinRequest (firstUncommittedSlot (nodeState n)) (currentTerm (nodeState n)) (lastAcceptedTermInSlot (nodeState n)) \<rangle>\<rightarrow> (OneNode n)".
+    from electionValueForced_max show " \<And>n n' a'. electionValueForced (nodeState n) \<Longrightarrow> \<not> (\<exists>x. \<langle> PublishRequest (firstUncommittedSlot (nodeState n)) (currentTerm (nodeState n)) x \<rangle>\<leadsto>) \<Longrightarrow> n' \<in> joinVotes (nodeState n) \<Longrightarrow> n' \<midarrow>\<langle> JoinRequest (firstUncommittedSlot (nodeState n)) (currentTerm (nodeState n)) a' \<rangle>\<rightarrow> (OneNode n) \<Longrightarrow> maxTermOption a' (lastAcceptedTermInSlot (nodeState n)) = lastAcceptedTermInSlot (nodeState n)".
     from publishVotes show "\<And>n n'. n' \<in> publishVotes (nodeState n) \<Longrightarrow> n' \<midarrow>\<langle> PublishResponse (firstUncommittedSlot (nodeState n)) (currentTerm (nodeState n)) \<rangle>\<leadsto>".
     from currentClusterState_lastCommittedClusterStateBefore show "\<And>n. currentClusterState (nodeState n) = lastCommittedClusterStateBefore (firstUncommittedSlot (nodeState n))".
     from joinVotes show "\<And>n n'. n' \<in> joinVotes (nodeState n) \<Longrightarrow> promised (firstUncommittedSlot (nodeState n)) n' n (currentTerm (nodeState n))".
@@ -602,7 +608,7 @@ proof -
     from currentVotingNodes_firstUncommittedSlot show "\<And>n. currentVotingNodes (nodeState n) = V (firstUncommittedSlot (nodeState n))".
     from publishVotes_currentVotingNodes show "\<And>n. publishVotes (nodeState n) \<subseteq> currentVotingNodes (nodeState n)".
     from firstUncommittedSlot_PublishRequest show "\<And>i n t x. firstUncommittedSlot (nodeState n) < i \<Longrightarrow> \<not> n \<midarrow>\<langle> PublishRequest i t x \<rangle>\<leadsto>".
-    from lastAcceptedTerm_Some_value show "\<And>n t. lastAcceptedTerm (nodeState n) = Some t \<Longrightarrow> \<langle> PublishRequest (firstUncommittedSlot (nodeState n)) t (lastAcceptedValue (nodeState n)) \<rangle>\<leadsto>".
+    from lastAcceptedTerm_Some_value show "\<And>n t. lastAcceptedTerm (nodeState n) = Some t \<Longrightarrow> \<langle> PublishRequest (lastAcceptedSlot (nodeState n)) t (lastAcceptedValue (nodeState n)) \<rangle>\<leadsto>".
     from PublishRequest_currentTerm show "\<And>n t x. n \<midarrow>\<langle> PublishRequest (firstUncommittedSlot (nodeState n)) t x \<rangle>\<leadsto> \<Longrightarrow> t \<le> currentTerm (nodeState n)".
     from PublishRequest_publishPermitted_currentTerm show "\<And>n t x. n \<midarrow>\<langle> PublishRequest (firstUncommittedSlot (nodeState n)) t x \<rangle>\<leadsto> \<Longrightarrow> publishPermitted (nodeState n) \<Longrightarrow> t < currentTerm (nodeState n)".
     from CatchUpResponse_committedTo show "\<And>i conf cs. \<langle> CatchUpResponse i conf cs \<rangle>\<leadsto> \<Longrightarrow> committed\<^sub>< i".
@@ -660,6 +666,8 @@ proof -
     "\<And>n. electionValueForced (nodeState' n) = electionValueForced (nodeState n)"
     "\<And>n. lastAcceptedTerm (nodeState' n) = lastAcceptedTerm (nodeState n)"
     "\<And>n. lastAcceptedValue (nodeState' n) = lastAcceptedValue (nodeState n)"
+    "\<And>n. lastAcceptedSlot (nodeState' n) = lastAcceptedSlot (nodeState n)"
+    "\<And>n. lastAcceptedTermInSlot (nodeState' n) = lastAcceptedTermInSlot (nodeState n)"
     by (unfold nodeState', auto)
 
   have v_eq[simp]: "v' = v" by (intro ext, auto simp add: v'_def v_def)
@@ -687,16 +695,17 @@ proof -
     from JoinRequest_unique_destination show "\<And>i' i s t a a' d d'. s \<midarrow>\<langle> JoinRequest i t a \<rangle>\<rightarrow> d \<Longrightarrow> s \<midarrow>\<langle> JoinRequest i' t a' \<rangle>\<rightarrow> d' \<Longrightarrow> d = d'".
     from currentNode_nodeState show "\<And>n. currentNode (nodeState n) = n" .
     from committedTo_firstUncommittedSlot show "\<And>n. committed\<^sub>< (firstUncommittedSlot (nodeState n))" .
-    from firstUncommittedSlot_PublishResponse show "\<And>n i t. firstUncommittedSlot (nodeState n) < i \<Longrightarrow> \<not> n \<midarrow>\<langle> PublishResponse i t \<rangle>\<leadsto>" .
-    from lastAcceptedTerm_None show "\<And>n t. lastAcceptedTerm (nodeState n) = None \<Longrightarrow> \<not> n \<midarrow>\<langle> PublishResponse (firstUncommittedSlot (nodeState n)) t \<rangle>\<leadsto>".
-    from lastAcceptedTerm_Some_sent show "\<And>n t. lastAcceptedTerm (nodeState n) = Some t \<Longrightarrow> n \<midarrow>\<langle> PublishResponse (firstUncommittedSlot (nodeState n)) t \<rangle>\<leadsto>".
-    from lastAcceptedTerm_Some_max show "\<And>n t t'. lastAcceptedTerm (nodeState n) = Some t \<Longrightarrow> n \<midarrow>\<langle> PublishResponse (firstUncommittedSlot (nodeState n)) t' \<rangle>\<leadsto> \<Longrightarrow> t' \<le> t".
+    from lastAcceptedSlot_firstUncommittedSlot  show "\<And>n. lastAcceptedSlot (nodeState n) \<le> firstUncommittedSlot (nodeState n)".
+    from lastAcceptedSlot_PublishResponse show "\<And>n i t. lastAcceptedSlot (nodeState n) < i \<Longrightarrow> \<not> n \<midarrow>\<langle> PublishResponse i t \<rangle>\<leadsto>" .
+    from lastAcceptedTerm_None show "\<And>n t. lastAcceptedTerm (nodeState n) = None \<Longrightarrow> \<not> n \<midarrow>\<langle> PublishResponse (lastAcceptedSlot (nodeState n)) t \<rangle>\<leadsto>".
+    from lastAcceptedTerm_Some_sent show "\<And>n t. lastAcceptedTerm (nodeState n) = Some t \<Longrightarrow> n \<midarrow>\<langle> PublishResponse (lastAcceptedSlot (nodeState n)) t \<rangle>\<leadsto>".
+    from lastAcceptedTerm_Some_max show "\<And>n t t'. lastAcceptedTerm (nodeState n) = Some t \<Longrightarrow> n \<midarrow>\<langle> PublishResponse (lastAcceptedSlot (nodeState n)) t' \<rangle>\<leadsto> \<Longrightarrow> t' \<le> t".
     from JoinRequest_currentTerm show "\<And>n i t a. n \<midarrow>\<langle> JoinRequest i t a \<rangle>\<leadsto> \<Longrightarrow> t \<le> currentTerm (nodeState n)".
     from JoinRequest_slot_function show "\<And>n i i' t a a'. n \<midarrow>\<langle> JoinRequest i t a \<rangle>\<leadsto> \<Longrightarrow> n \<midarrow>\<langle> JoinRequest i' t a' \<rangle>\<leadsto> \<Longrightarrow> i = i'".
     from electionWon_isQuorum show "\<And>n. electionWon (nodeState n) \<Longrightarrow> isQuorum (nodeState n) (joinVotes (nodeState n))".
     from electionValueFree_JoinRequest show "\<And>n n'. \<not> electionValueForced (nodeState n) \<Longrightarrow> n' \<in> joinVotes (nodeState n) \<Longrightarrow> n' \<midarrow>\<langle> JoinRequest (firstUncommittedSlot (nodeState n)) (currentTerm (nodeState n)) None \<rangle>\<rightarrow> (OneNode n) \<or> (\<exists>i<firstUncommittedSlot (nodeState n). \<exists>a. n' \<midarrow>\<langle> JoinRequest i (currentTerm (nodeState n)) a \<rangle>\<rightarrow> (OneNode n))".
-    from electionValueForced_JoinRequest show "\<And>n. electionValueForced (nodeState n) \<Longrightarrow> \<not> (\<exists>x. \<langle> PublishRequest (firstUncommittedSlot (nodeState n)) (currentTerm (nodeState n)) x \<rangle>\<leadsto>) \<Longrightarrow> \<exists>n'\<in>joinVotes (nodeState n). n' \<midarrow>\<langle> JoinRequest (firstUncommittedSlot (nodeState n)) (currentTerm (nodeState n)) (lastAcceptedTerm (nodeState n)) \<rangle>\<rightarrow> (OneNode n)".
-    from electionValueForced_max show " \<And>n n' a'. electionValueForced (nodeState n) \<Longrightarrow> \<not> (\<exists>x. \<langle> PublishRequest (firstUncommittedSlot (nodeState n)) (currentTerm (nodeState n)) x \<rangle>\<leadsto>) \<Longrightarrow> n' \<in> joinVotes (nodeState n) \<Longrightarrow> n' \<midarrow>\<langle> JoinRequest (firstUncommittedSlot (nodeState n)) (currentTerm (nodeState n)) a' \<rangle>\<rightarrow> (OneNode n) \<Longrightarrow> maxTermOption a' (lastAcceptedTerm (nodeState n)) = lastAcceptedTerm (nodeState n)".
+    from electionValueForced_JoinRequest show "\<And>n. electionValueForced (nodeState n) \<Longrightarrow> \<not> (\<exists>x. \<langle> PublishRequest (firstUncommittedSlot (nodeState n)) (currentTerm (nodeState n)) x \<rangle>\<leadsto>) \<Longrightarrow> \<exists>n'\<in>joinVotes (nodeState n). n' \<midarrow>\<langle> JoinRequest (firstUncommittedSlot (nodeState n)) (currentTerm (nodeState n)) (lastAcceptedTermInSlot (nodeState n)) \<rangle>\<rightarrow> (OneNode n)".
+    from electionValueForced_max show " \<And>n n' a'. electionValueForced (nodeState n) \<Longrightarrow> \<not> (\<exists>x. \<langle> PublishRequest (firstUncommittedSlot (nodeState n)) (currentTerm (nodeState n)) x \<rangle>\<leadsto>) \<Longrightarrow> n' \<in> joinVotes (nodeState n) \<Longrightarrow> n' \<midarrow>\<langle> JoinRequest (firstUncommittedSlot (nodeState n)) (currentTerm (nodeState n)) a' \<rangle>\<rightarrow> (OneNode n) \<Longrightarrow> maxTermOption a' (lastAcceptedTermInSlot (nodeState n)) = lastAcceptedTermInSlot (nodeState n)".
     from publishVotes show "\<And>n n'. n' \<in> publishVotes (nodeState n) \<Longrightarrow> n' \<midarrow>\<langle> PublishResponse (firstUncommittedSlot (nodeState n)) (currentTerm (nodeState n)) \<rangle>\<leadsto>".
     from publishVotes_currentVotingNodes show "\<And>n. publishVotes (nodeState n) \<subseteq> currentVotingNodes (nodeState n)".
     from currentClusterState_lastCommittedClusterStateBefore show "\<And>n. currentClusterState (nodeState n) = lastCommittedClusterStateBefore (firstUncommittedSlot (nodeState n))".
@@ -708,7 +717,7 @@ proof -
     from ApplyCommit_quorum show "\<And>i t. \<langle> ApplyCommit i t \<rangle>\<leadsto> \<Longrightarrow> \<exists>q\<in>majorities (V i). \<forall>s\<in>q. s \<midarrow>\<langle> PublishResponse i t \<rangle>\<leadsto>".
     from currentVotingNodes_firstUncommittedSlot show "\<And>n. currentVotingNodes (nodeState n) = V (firstUncommittedSlot (nodeState n))".
     from firstUncommittedSlot_PublishRequest show "\<And>i n t x. firstUncommittedSlot (nodeState n) < i \<Longrightarrow> \<not> n \<midarrow>\<langle> PublishRequest i t x \<rangle>\<leadsto>".
-    from lastAcceptedTerm_Some_value show "\<And>n t. lastAcceptedTerm (nodeState n) = Some t \<Longrightarrow> \<langle> PublishRequest (firstUncommittedSlot (nodeState n)) t (lastAcceptedValue (nodeState n)) \<rangle>\<leadsto>".
+    from lastAcceptedTerm_Some_value show "\<And>n t. lastAcceptedTerm (nodeState n) = Some t \<Longrightarrow> \<langle> PublishRequest (lastAcceptedSlot (nodeState n)) t (lastAcceptedValue (nodeState n)) \<rangle>\<leadsto>".
     from PublishRequest_currentTerm show "\<And>n t x. n \<midarrow>\<langle> PublishRequest (firstUncommittedSlot (nodeState n)) t x \<rangle>\<leadsto> \<Longrightarrow> t \<le> currentTerm (nodeState n)".
     from PublishRequest_publishPermitted_currentTerm show "\<And>n t x. n \<midarrow>\<langle> PublishRequest (firstUncommittedSlot (nodeState n)) t x \<rangle>\<leadsto> \<Longrightarrow> publishPermitted (nodeState n) \<Longrightarrow> t < currentTerm (nodeState n)".
     from CatchUpResponse_committedTo show "\<And>i conf cs. \<langle> CatchUpResponse i conf cs \<rangle>\<leadsto> \<Longrightarrow> committed\<^sub>< i".
@@ -770,6 +779,8 @@ next
     "\<And>n q. isQuorum (nodeState' n) q = isQuorum (nodeState n) q"
     "\<And>n. lastAcceptedTerm (nodeState' n) = lastAcceptedTerm (nodeState n)"
     "\<And>n. lastAcceptedValue (nodeState' n) = lastAcceptedValue (nodeState n)"
+    "\<And>n. lastAcceptedSlot (nodeState' n) = lastAcceptedSlot (nodeState n)"
+    "\<And>n. lastAcceptedTermInSlot (nodeState' n) = lastAcceptedTermInSlot (nodeState n)"
     "currentTerm (nodeState' n\<^sub>0) = t"
     "electionWon (nodeState' n\<^sub>0) = False"
     "joinVotes (nodeState' n\<^sub>0) = {}"
@@ -777,7 +788,7 @@ next
     "publishPermitted (nodeState' n\<^sub>0) = True"
     "publishVotes (nodeState' n\<^sub>0) = {}"
     using t
-    by (unfold nodeState'_def, auto simp add: nd_def isQuorum_def nd' ensureCurrentTerm_def)
+    by (unfold nodeState'_def, auto simp add: nd_def isQuorum_def nd' ensureCurrentTerm_def lastAcceptedTermInSlot_def)
 
   have currentTerm_increases: "\<And>n. currentTerm (nodeState n) \<le> currentTerm (nodeState' n)"
     using nd_def nodeState'_def property_simps t by auto
@@ -807,10 +818,11 @@ next
     from JoinRequest_unique_destination show "\<And>i' i s t a a' d d'. s \<midarrow>\<langle> JoinRequest i t a \<rangle>\<rightarrow> d \<Longrightarrow> s \<midarrow>\<langle> JoinRequest i' t a' \<rangle>\<rightarrow> d' \<Longrightarrow> d = d'".
     from currentNode_nodeState show "\<And>n. currentNode (nodeState n) = n" .
     from committedTo_firstUncommittedSlot show "\<And>n. committed\<^sub>< (firstUncommittedSlot (nodeState n))" .
-    from firstUncommittedSlot_PublishResponse show "\<And>n i t. firstUncommittedSlot (nodeState n) < i \<Longrightarrow> \<not> n \<midarrow>\<langle> PublishResponse i t \<rangle>\<leadsto>" .
-    from lastAcceptedTerm_None show "\<And>n t. lastAcceptedTerm (nodeState n) = None \<Longrightarrow> \<not> n \<midarrow>\<langle> PublishResponse (firstUncommittedSlot (nodeState n)) t \<rangle>\<leadsto>".
-    from lastAcceptedTerm_Some_sent show "\<And>n t. lastAcceptedTerm (nodeState n) = Some t \<Longrightarrow> n \<midarrow>\<langle> PublishResponse (firstUncommittedSlot (nodeState n)) t \<rangle>\<leadsto>".
-    from lastAcceptedTerm_Some_max show "\<And>n t t'. lastAcceptedTerm (nodeState n) = Some t \<Longrightarrow> n \<midarrow>\<langle> PublishResponse (firstUncommittedSlot (nodeState n)) t' \<rangle>\<leadsto> \<Longrightarrow> t' \<le> t".
+    from lastAcceptedSlot_firstUncommittedSlot  show "\<And>n. lastAcceptedSlot (nodeState n) \<le> firstUncommittedSlot (nodeState n)".
+    from lastAcceptedSlot_PublishResponse show "\<And>n i t. lastAcceptedSlot (nodeState n) < i \<Longrightarrow> \<not> n \<midarrow>\<langle> PublishResponse i t \<rangle>\<leadsto>" .
+    from lastAcceptedTerm_None show "\<And>n t. lastAcceptedTerm (nodeState n) = None \<Longrightarrow> \<not> n \<midarrow>\<langle> PublishResponse (lastAcceptedSlot (nodeState n)) t \<rangle>\<leadsto>".
+    from lastAcceptedTerm_Some_sent show "\<And>n t. lastAcceptedTerm (nodeState n) = Some t \<Longrightarrow> n \<midarrow>\<langle> PublishResponse (lastAcceptedSlot (nodeState n)) t \<rangle>\<leadsto>".
+    from lastAcceptedTerm_Some_max show "\<And>n t t'. lastAcceptedTerm (nodeState n) = Some t \<Longrightarrow> n \<midarrow>\<langle> PublishResponse (lastAcceptedSlot (nodeState n)) t' \<rangle>\<leadsto> \<Longrightarrow> t' \<le> t".
     from JoinRequest_slot_function show "\<And>n i i' t a a'. n \<midarrow>\<langle> JoinRequest i t a \<rangle>\<leadsto> \<Longrightarrow> n \<midarrow>\<langle> JoinRequest i' t a' \<rangle>\<leadsto> \<Longrightarrow> i = i'".
     from currentClusterState_lastCommittedClusterStateBefore show "\<And>n. currentClusterState (nodeState n) = lastCommittedClusterStateBefore (firstUncommittedSlot (nodeState n))".
     from PublishRequest_committedTo show "\<And>i t x. \<langle> PublishRequest i t x \<rangle>\<leadsto> \<Longrightarrow> committed\<^sub>< i".
@@ -819,7 +831,7 @@ next
     from ApplyCommit_quorum show "\<And>i t. \<langle> ApplyCommit i t \<rangle>\<leadsto> \<Longrightarrow> \<exists>q\<in>majorities (V i). \<forall>s\<in>q. s \<midarrow>\<langle> PublishResponse i t \<rangle>\<leadsto>".
     from currentVotingNodes_firstUncommittedSlot show "\<And>n. currentVotingNodes (nodeState n) = V (firstUncommittedSlot (nodeState n))".
     from firstUncommittedSlot_PublishRequest show "\<And>i n t x. firstUncommittedSlot (nodeState n) < i \<Longrightarrow> \<not> n \<midarrow>\<langle> PublishRequest i t x \<rangle>\<leadsto>".
-    from lastAcceptedTerm_Some_value show "\<And>n t. lastAcceptedTerm (nodeState n) = Some t \<Longrightarrow> \<langle> PublishRequest (firstUncommittedSlot (nodeState n)) t (lastAcceptedValue (nodeState n)) \<rangle>\<leadsto>".
+    from lastAcceptedTerm_Some_value show "\<And>n t. lastAcceptedTerm (nodeState n) = Some t \<Longrightarrow> \<langle> PublishRequest (lastAcceptedSlot (nodeState n)) t (lastAcceptedValue (nodeState n)) \<rangle>\<leadsto>".
     from PublishRequest_quorum show "\<And>i s t x. s \<midarrow>\<langle> PublishRequest i t x \<rangle>\<leadsto> \<Longrightarrow> \<exists>q\<in>majorities (V i). (\<forall>n\<in>q. promised i n s t) \<and> (prevAccepted i t q = {} \<or> v i t = v i (maxTerm (prevAccepted i t q)))".
     from CatchUpResponse_committedTo show "\<And>i conf cs. \<langle> CatchUpResponse i conf cs \<rangle>\<leadsto> \<Longrightarrow> committed\<^sub>< i".
     from CatchUpResponse_V show "\<And>i conf cs. \<langle> CatchUpResponse i conf cs \<rangle>\<leadsto> \<Longrightarrow> V i = conf".
@@ -850,7 +862,7 @@ next
       unfolding nodeState'_def by (auto simp add: nd'_def, blast)
 
     from electionValueForced_JoinRequest
-    show "\<And>n. electionValueForced (nodeState' n) \<Longrightarrow> \<not> (\<exists>x. \<langle> PublishRequest (firstUncommittedSlot (nodeState n)) (currentTerm (nodeState' n)) x \<rangle>\<leadsto>) \<Longrightarrow> \<exists>n'\<in>joinVotes (nodeState' n). n' \<midarrow>\<langle> JoinRequest (firstUncommittedSlot (nodeState n)) (currentTerm (nodeState' n)) (lastAcceptedTerm (nodeState n)) \<rangle>\<rightarrow> (OneNode n)"
+    show "\<And>n. electionValueForced (nodeState' n) \<Longrightarrow> \<not> (\<exists>x. \<langle> PublishRequest (firstUncommittedSlot (nodeState n)) (currentTerm (nodeState' n)) x \<rangle>\<leadsto>) \<Longrightarrow> \<exists>n'\<in>joinVotes (nodeState' n). n' \<midarrow>\<langle> JoinRequest (firstUncommittedSlot (nodeState n)) (currentTerm (nodeState' n)) (lastAcceptedTermInSlot (nodeState n)) \<rangle>\<rightarrow> (OneNode n)"
       unfolding nodeState'_def by (auto simp add: nd'_def)
 
     from electionWon_isQuorum show "\<And>n. electionWon (nodeState' n) \<Longrightarrow> isQuorum (nodeState n) (joinVotes (nodeState' n))"
@@ -858,7 +870,7 @@ next
 
     fix n
     from electionValueForced_max
-    show "\<And>n' a'. electionValueForced (nodeState' n) \<Longrightarrow> \<not> (\<exists>x. \<langle> PublishRequest (firstUncommittedSlot (nodeState n)) (currentTerm (nodeState' n)) x \<rangle>\<leadsto>) \<Longrightarrow> n' \<in> joinVotes (nodeState' n) \<Longrightarrow> n' \<midarrow>\<langle> JoinRequest (firstUncommittedSlot (nodeState n)) (currentTerm (nodeState' n)) a' \<rangle>\<rightarrow> (OneNode n) \<Longrightarrow> maxTermOption a' (lastAcceptedTerm (nodeState n)) = lastAcceptedTerm (nodeState n)"
+    show "\<And>n' a'. electionValueForced (nodeState' n) \<Longrightarrow> \<not> (\<exists>x. \<langle> PublishRequest (firstUncommittedSlot (nodeState n)) (currentTerm (nodeState' n)) x \<rangle>\<leadsto>) \<Longrightarrow> n' \<in> joinVotes (nodeState' n) \<Longrightarrow> n' \<midarrow>\<langle> JoinRequest (firstUncommittedSlot (nodeState n)) (currentTerm (nodeState' n)) a' \<rangle>\<rightarrow> (OneNode n) \<Longrightarrow> maxTermOption a' (lastAcceptedTermInSlot (nodeState n)) = lastAcceptedTermInSlot (nodeState n)"
       unfolding nodeState'_def by (cases "n = n\<^sub>0", auto simp add: nd'_def)
 
     from lastAcceptedTerm_Some_currentTerm currentTerm_increases
@@ -871,15 +883,19 @@ next
 qed
 
 lemma (in zenStep) sendJoinRequest_invariants:
-  assumes messages': "messages' = sendTo (OneNode d\<^sub>0) (nd'', Some (JoinRequest (firstUncommittedSlot nd) (currentTerm nd) (lastAcceptedTerm nd)))"
+  assumes messages': "messages' = sendTo (OneNode d\<^sub>0) (nd'',
+    Some (JoinRequest (firstUncommittedSlot nd) (currentTerm nd)
+                      (if lastAcceptedSlot nd = firstUncommittedSlot nd then lastAcceptedTerm nd else None)))"
   assumes nd': "nd' = nd"
   assumes not_sent: "\<And>i a. \<not> n\<^sub>0 \<midarrow>\<langle> JoinRequest i (currentTerm nd) a \<rangle>\<leadsto>"
   assumes not_accepted: "\<And>t'. lastAcceptedTerm nd = Some t' \<Longrightarrow> t' < currentTerm nd"
   shows "zen messages' nodeState'"
 proof -
+  define promisedTerm where "promisedTerm \<equiv> if lastAcceptedSlot nd = firstUncommittedSlot nd then lastAcceptedTerm nd else None"
+
   have messages': "messages' = insert \<lparr>sender = n\<^sub>0, destination = OneNode d\<^sub>0,
-                       payload = JoinRequest (firstUncommittedSlot nd) (currentTerm nd) (lastAcceptedTerm nd)\<rparr> messages"
-    by (simp add: messages')
+                       payload = JoinRequest (firstUncommittedSlot nd) (currentTerm nd) promisedTerm\<rparr> messages"
+    by (simp add: messages' promisedTerm_def)
 
   have nodeState'[simp]: "nodeState' = nodeState"
     by (intro ext, auto simp add: nodeState'_def nd' nd_def)
@@ -907,16 +923,16 @@ proof -
   have JoinRequest':
     "\<And>s d i t' a. (s \<midarrow>\<langle> JoinRequest i t' a \<rangle>\<rightarrow>' d) =
     ((s \<midarrow>\<langle> JoinRequest i t' a \<rangle>\<rightarrow> d)
-      \<or> (s, i, t', a, d) = (n\<^sub>0, firstUncommittedSlot nd, currentTerm nd, lastAcceptedTerm nd, OneNode d\<^sub>0))"
+      \<or> (s, i, t', a, d) = (n\<^sub>0, firstUncommittedSlot nd, currentTerm nd, promisedTerm, OneNode d\<^sub>0))"
     "\<And>d i t' a. (\<langle> JoinRequest i t' a \<rangle>\<rightarrow>' d) =
     ((\<langle> JoinRequest i t' a \<rangle>\<rightarrow> d)
-      \<or> (i, t', a, d) = (firstUncommittedSlot nd, currentTerm nd, lastAcceptedTerm nd, OneNode d\<^sub>0))"
+      \<or> (i, t', a, d) = (firstUncommittedSlot nd, currentTerm nd, promisedTerm, OneNode d\<^sub>0))"
     "\<And>s i t' a. (s \<midarrow>\<langle> JoinRequest i t' a \<rangle>\<leadsto>') =
     ((s \<midarrow>\<langle> JoinRequest i t' a \<rangle>\<leadsto>)
-      \<or> (s, i, t', a) = (n\<^sub>0, firstUncommittedSlot nd, currentTerm nd, lastAcceptedTerm nd))"
+      \<or> (s, i, t', a) = (n\<^sub>0, firstUncommittedSlot nd, currentTerm nd, promisedTerm))"
     "\<And>i t' a. (\<langle> JoinRequest i t' a \<rangle>\<leadsto>') =
     ((\<langle> JoinRequest i t' a \<rangle>\<leadsto>)
-      \<or> (i, t', a) = (firstUncommittedSlot nd, currentTerm nd, lastAcceptedTerm nd))"
+      \<or> (i, t', a) = (firstUncommittedSlot nd, currentTerm nd, promisedTerm))"
     by (unfold isMessageFromTo'_def isMessageFromTo_def isMessageTo'_def isMessageTo_def
         isMessageFrom'_def isMessageFrom_def isMessage'_def isMessage_def, auto simp add: messages')
 
@@ -931,7 +947,7 @@ proof -
   have promised_eq: "\<And>i s dn t. promised' i s dn t = (promised i s dn t \<or> (firstUncommittedSlot nd \<le> i \<and> s = n\<^sub>0 \<and> dn = d\<^sub>0 \<and> t = currentTerm nd))"
     unfolding promised'_def promised_def JoinRequest' by auto
 
-  have prevAccepted_eq: "\<And>i t q. prevAccepted' i t q = prevAccepted i t q \<union> {t'. n\<^sub>0 \<in> q \<and> i = firstUncommittedSlot nd \<and> t = currentTerm nd \<and> lastAcceptedTerm nd = Some t'}"
+  have prevAccepted_eq: "\<And>i t q. prevAccepted' i t q = prevAccepted i t q \<union> {t'. n\<^sub>0 \<in> q \<and> i = firstUncommittedSlot nd \<and> t = currentTerm nd \<and> promisedTerm = Some t'}"
     unfolding prevAccepted_def prevAccepted'_def JoinRequest' by auto
 
   have property_simps[simp]:
@@ -941,6 +957,8 @@ proof -
     "\<And>n q. isQuorum (nodeState' n) q = isQuorum (nodeState n) q"
     "\<And>n. lastAcceptedTerm (nodeState' n) = lastAcceptedTerm (nodeState n)"
     "\<And>n. lastAcceptedValue (nodeState' n) = lastAcceptedValue (nodeState n)"
+    "\<And>n. lastAcceptedSlot (nodeState' n) = lastAcceptedSlot (nodeState n)"
+    "\<And>n. lastAcceptedTermInSlot (nodeState' n) = lastAcceptedTermInSlot (nodeState n)"
     "\<And>n. currentTerm (nodeState' n) = currentTerm (nodeState n)"
     "\<And>n. publishPermitted (nodeState' n) = publishPermitted (nodeState n)"
     "\<And>n. publishVotes (nodeState' n) = publishVotes (nodeState n)"
@@ -957,10 +975,11 @@ proof -
   from finite_messages show "finite messages'" by (simp add: messages')
     from currentNode_nodeState show "\<And>n. currentNode (nodeState n) = n" .
     from committedTo_firstUncommittedSlot show "\<And>n. committed\<^sub>< (firstUncommittedSlot (nodeState n))" .
-    from firstUncommittedSlot_PublishResponse show "\<And>n i t. firstUncommittedSlot (nodeState n) < i \<Longrightarrow> \<not> n \<midarrow>\<langle> PublishResponse i t \<rangle>\<leadsto>" .
-    from lastAcceptedTerm_None show "\<And>n t. lastAcceptedTerm (nodeState n) = None \<Longrightarrow> \<not> n \<midarrow>\<langle> PublishResponse (firstUncommittedSlot (nodeState n)) t \<rangle>\<leadsto>".
-    from lastAcceptedTerm_Some_sent show "\<And>n t. lastAcceptedTerm (nodeState n) = Some t \<Longrightarrow> n \<midarrow>\<langle> PublishResponse (firstUncommittedSlot (nodeState n)) t \<rangle>\<leadsto>".
-    from lastAcceptedTerm_Some_max show "\<And>n t t'. lastAcceptedTerm (nodeState n) = Some t \<Longrightarrow> n \<midarrow>\<langle> PublishResponse (firstUncommittedSlot (nodeState n)) t' \<rangle>\<leadsto> \<Longrightarrow> t' \<le> t".
+    from lastAcceptedSlot_firstUncommittedSlot  show "\<And>n. lastAcceptedSlot (nodeState n) \<le> firstUncommittedSlot (nodeState n)".
+    from lastAcceptedSlot_PublishResponse show "\<And>n i t. lastAcceptedSlot (nodeState n) < i \<Longrightarrow> \<not> n \<midarrow>\<langle> PublishResponse i t \<rangle>\<leadsto>" .
+    from lastAcceptedTerm_None show "\<And>n t. lastAcceptedTerm (nodeState n) = None \<Longrightarrow> \<not> n \<midarrow>\<langle> PublishResponse (lastAcceptedSlot (nodeState n)) t \<rangle>\<leadsto>".
+    from lastAcceptedTerm_Some_sent show "\<And>n t. lastAcceptedTerm (nodeState n) = Some t \<Longrightarrow> n \<midarrow>\<langle> PublishResponse (lastAcceptedSlot (nodeState n)) t \<rangle>\<leadsto>".
+    from lastAcceptedTerm_Some_max show "\<And>n t t'. lastAcceptedTerm (nodeState n) = Some t \<Longrightarrow> n \<midarrow>\<langle> PublishResponse (lastAcceptedSlot (nodeState n)) t' \<rangle>\<leadsto> \<Longrightarrow> t' \<le> t".
     from electionWon_isQuorum show "\<And>n. electionWon (nodeState n) \<Longrightarrow> isQuorum (nodeState n) (joinVotes (nodeState n))".
     from publishVotes show "\<And>n n'. n' \<in> publishVotes (nodeState n) \<Longrightarrow> n' \<midarrow>\<langle> PublishResponse (firstUncommittedSlot (nodeState n)) (currentTerm (nodeState n)) \<rangle>\<leadsto>".
     from publishVotes_currentVotingNodes show "\<And>n. publishVotes (nodeState n) \<subseteq> currentVotingNodes (nodeState n)".
@@ -971,7 +990,7 @@ proof -
     from ApplyCommit_quorum show "\<And>i t. \<langle> ApplyCommit i t \<rangle>\<leadsto> \<Longrightarrow> \<exists>q\<in>majorities (V i). \<forall>s\<in>q. s \<midarrow>\<langle> PublishResponse i t \<rangle>\<leadsto>".
     from currentVotingNodes_firstUncommittedSlot show "\<And>n. currentVotingNodes (nodeState n) = V (firstUncommittedSlot (nodeState n))".
     from firstUncommittedSlot_PublishRequest show "\<And>i n t x. firstUncommittedSlot (nodeState n) < i \<Longrightarrow> \<not> n \<midarrow>\<langle> PublishRequest i t x \<rangle>\<leadsto>".
-    from lastAcceptedTerm_Some_value show "\<And>n t. lastAcceptedTerm (nodeState n) = Some t \<Longrightarrow> \<langle> PublishRequest (firstUncommittedSlot (nodeState n)) t (lastAcceptedValue (nodeState n)) \<rangle>\<leadsto>".
+    from lastAcceptedTerm_Some_value show "\<And>n t. lastAcceptedTerm (nodeState n) = Some t \<Longrightarrow> \<langle> PublishRequest (lastAcceptedSlot (nodeState n)) t (lastAcceptedValue (nodeState n)) \<rangle>\<leadsto>".
     from PublishRequest_currentTerm show "\<And>n t x. n \<midarrow>\<langle> PublishRequest (firstUncommittedSlot (nodeState n)) t x \<rangle>\<leadsto> \<Longrightarrow> t \<le> currentTerm (nodeState n)".
     from PublishRequest_publishPermitted_currentTerm show "\<And>n t x. n \<midarrow>\<langle> PublishRequest (firstUncommittedSlot (nodeState n)) t x \<rangle>\<leadsto> \<Longrightarrow> publishPermitted (nodeState n) \<Longrightarrow> t < currentTerm (nodeState n)".
     from CatchUpResponse_committedTo show "\<And>i conf cs. \<langle> CatchUpResponse i conf cs \<rangle>\<leadsto> \<Longrightarrow> committed\<^sub>< i".
@@ -985,27 +1004,32 @@ proof -
     from electionValueFree_JoinRequest show "\<And>n n'. \<not> electionValueForced (nodeState n) \<Longrightarrow> n' \<in> joinVotes (nodeState n) \<Longrightarrow> n' \<midarrow>\<langle> JoinRequest (firstUncommittedSlot (nodeState n)) (currentTerm (nodeState n)) None \<rangle>\<rightarrow>' (OneNode n) \<or> (\<exists>i<firstUncommittedSlot (nodeState n). \<exists>a. n' \<midarrow>\<langle> JoinRequest i (currentTerm (nodeState n)) a \<rangle>\<rightarrow>' (OneNode n))"
       unfolding JoinRequest' by (auto simp add: nd_def)
 
-    from electionValueForced_JoinRequest show "\<And>n. electionValueForced (nodeState n) \<Longrightarrow> \<not> (\<exists>x. \<langle> PublishRequest (firstUncommittedSlot (nodeState n)) (currentTerm (nodeState n)) x \<rangle>\<leadsto>) \<Longrightarrow> \<exists>n'\<in>joinVotes (nodeState n). n' \<midarrow>\<langle> JoinRequest (firstUncommittedSlot (nodeState n)) (currentTerm (nodeState n)) (lastAcceptedTerm (nodeState n)) \<rangle>\<rightarrow>' (OneNode n)"
+    from electionValueForced_JoinRequest show "\<And>n. electionValueForced (nodeState n) \<Longrightarrow> \<not> (\<exists>x. \<langle> PublishRequest (firstUncommittedSlot (nodeState n)) (currentTerm (nodeState n)) x \<rangle>\<leadsto>) \<Longrightarrow> \<exists>n'\<in>joinVotes (nodeState n). n' \<midarrow>\<langle> JoinRequest (firstUncommittedSlot (nodeState n)) (currentTerm (nodeState n)) (lastAcceptedTermInSlot (nodeState n)) \<rangle>\<rightarrow>' (OneNode n)"
       unfolding JoinRequest' by (auto simp add: nd_def)
 
     from joinVotes show "\<And>n n'. n' \<in> joinVotes (nodeState n) \<Longrightarrow> promised' (firstUncommittedSlot (nodeState n)) n' n (currentTerm (nodeState n))"
       unfolding promised_eq by simp
 
-    from JoinRequest_future firstUncommittedSlot_PublishResponse
+    from JoinRequest_future lastAcceptedSlot_PublishResponse lastAcceptedSlot_firstUncommittedSlot
     show "\<And>i i' s t t' a. s \<midarrow>\<langle> JoinRequest i t a \<rangle>\<leadsto>' \<Longrightarrow> i < i' \<Longrightarrow> t' < t \<Longrightarrow> \<not> s \<midarrow>\<langle> PublishResponse i' t' \<rangle>\<leadsto>"
-      unfolding JoinRequest' by (auto simp add: nd_def)
+      unfolding JoinRequest' nd_def
+      by (smt Pair_inject le_imp_less_Suc le_trans nat_less_le not_less_eq)
 
     from JoinRequest_None show "\<And>i s t t'. s \<midarrow>\<langle> JoinRequest i t None \<rangle>\<leadsto>' \<Longrightarrow> t' < t \<Longrightarrow> \<not> s \<midarrow>\<langle> PublishResponse i t' \<rangle>\<leadsto>"
-      unfolding JoinRequest' using lastAcceptedTerm_None nd' nd'_def by auto
+      unfolding JoinRequest' promisedTerm_def using JoinRequest_future lastAcceptedTerm_None lastAcceptedSlot_firstUncommittedSlot nd' nd'_def
+      by (smt Pair_inject \<open>\<And>t na ia. lastAcceptedSlot (nodeState na) < ia \<Longrightarrow> \<not> na \<midarrow>\<langle> PublishResponse ia t \<rangle>\<leadsto>\<close> le_less nodeState')
 
     from JoinRequest_Some_lt show "\<And>i s t t'. s \<midarrow>\<langle> JoinRequest i t (Some t') \<rangle>\<leadsto>' \<Longrightarrow> t' < t"
-      unfolding JoinRequest' using not_accepted by auto
+      unfolding JoinRequest' promisedTerm_def using not_accepted
+      by (smt fst_conv option.distinct(1) snd_conv)
 
     from JoinRequest_Some_PublishResponse show "\<And>i s t t'. s \<midarrow>\<langle> JoinRequest i t (Some t') \<rangle>\<leadsto>' \<Longrightarrow> s \<midarrow>\<langle> PublishResponse i t' \<rangle>\<leadsto>"
-      unfolding JoinRequest' using lastAcceptedTerm_Some_sent nd' nd'_def by auto
+      unfolding JoinRequest' promisedTerm_def using lastAcceptedTerm_Some_sent nd' nd'_def nd_def
+      by (smt Pair_inject option.distinct(1))
 
     from JoinRequest_Some_max show "\<And>i s t t' t''. s \<midarrow>\<langle> JoinRequest i t (Some t') \<rangle>\<leadsto>' \<Longrightarrow> t' < t'' \<Longrightarrow> t'' < t \<Longrightarrow> \<not> s \<midarrow>\<langle> PublishResponse i t'' \<rangle>\<leadsto>"
-      unfolding JoinRequest' by (metis Pair_inject lastAcceptedTerm_Some_max leD nd_def)
+      unfolding JoinRequest' promisedTerm_def nd_def
+      by (smt Pair_inject \<open>\<And>t' t na. \<lbrakk>lastAcceptedTerm (nodeState na) = Some t; na \<midarrow>\<langle> PublishResponse (lastAcceptedSlot (nodeState na)) t' \<rangle>\<leadsto>\<rbrakk> \<Longrightarrow> t' \<le> t\<close> leD option.discI)
 
     from JoinRequest_not_broadcast show "\<And>i t a d. \<langle> JoinRequest i t a \<rangle>\<rightarrow>' d \<Longrightarrow> d \<noteq> Broadcast"
       unfolding JoinRequest' by blast
@@ -1017,7 +1041,7 @@ proof -
       unfolding JoinRequest'
       by (metis JoinRequest'(3) Message.inject(2) RoutedMessage.ext_inject insert_iff isMessageFrom'_def isMessageFromTo'_def isMessageFromTo_def isMessageFrom_def messages' not_sent)
 
-    from electionValueForced_max show " \<And>n n' a'. electionValueForced (nodeState n) \<Longrightarrow> \<not> (\<exists>x. \<langle> PublishRequest (firstUncommittedSlot (nodeState n)) (currentTerm (nodeState n)) x \<rangle>\<leadsto>) \<Longrightarrow> n' \<in> joinVotes (nodeState n) \<Longrightarrow> n' \<midarrow>\<langle> JoinRequest (firstUncommittedSlot (nodeState n)) (currentTerm (nodeState n)) a' \<rangle>\<rightarrow>' (OneNode n) \<Longrightarrow> maxTermOption a' (lastAcceptedTerm (nodeState n)) = lastAcceptedTerm (nodeState n)"
+    from electionValueForced_max show " \<And>n n' a'. electionValueForced (nodeState n) \<Longrightarrow> \<not> (\<exists>x. \<langle> PublishRequest (firstUncommittedSlot (nodeState n)) (currentTerm (nodeState n)) x \<rangle>\<leadsto>) \<Longrightarrow> n' \<in> joinVotes (nodeState n) \<Longrightarrow> n' \<midarrow>\<langle> JoinRequest (firstUncommittedSlot (nodeState n)) (currentTerm (nodeState n)) a' \<rangle>\<rightarrow>' (OneNode n) \<Longrightarrow> maxTermOption a' (lastAcceptedTermInSlot (nodeState n)) = lastAcceptedTermInSlot (nodeState n)"
       unfolding JoinRequest'
       by (smt JoinRequest'(1) Message.inject(2) RoutedMessage.ext_inject insert_iff isMessageFromTo'_def isMessageFrom_def joinVotes messages' not_sent promised_def zen.JoinRequest_slot_function zenMessages.JoinRequest_value_function zenMessages_axioms zen_axioms)
 
@@ -1051,7 +1075,7 @@ next
   case True
   hence new_term: "currentTerm nd < t" by simp
 
-  have result: "result = (ensureCurrentTerm t nd, Some (JoinRequest (firstUncommittedSlot nd) t (lastAcceptedTerm nd)))"
+  have result: "result = (ensureCurrentTerm t nd, Some (JoinRequest (firstUncommittedSlot nd) t (lastAcceptedTermInSlot nd)))"
     by (simp add: result_def handleStartJoin_def True)
 
   have nd': "nd' = ensureCurrentTerm t nd" by (simp add: nd' result)
@@ -1079,14 +1103,16 @@ next
 
   have [simp]: "firstUncommittedSlot nd' = firstUncommittedSlot nd"
     "lastAcceptedTerm nd' = lastAcceptedTerm nd"
-    by (auto simp add: nd' ensureCurrentTerm_def)
+    "lastAcceptedSlot nd' = lastAcceptedSlot nd"
+    "lastAcceptedTermInSlot nd' = lastAcceptedTermInSlot nd"
+    by (auto simp add: nd' ensureCurrentTerm_def lastAcceptedTermInSlot_def)
 
   show "zen messages' nodeState'"
-  proof (intro zenStep.sendJoinRequest_invariants [OF zenStep1], unfold nd'_eq currentTerm_nd', simp_all add: messages' result)
+  proof (intro zenStep.sendJoinRequest_invariants [OF zenStep1], unfold nd'_eq currentTerm_nd', simp_all add: messages' result lastAcceptedTermInSlot_def)
     show "\<And>i a. \<forall>d. \<lparr>sender = n\<^sub>0, destination = d, payload = JoinRequest i t a\<rparr> \<notin> messages"
       using nd_def new_term zen.JoinRequest_currentTerm zen_axioms by fastforce
     show "\<And>t'. lastAcceptedTerm nd = Some t' \<Longrightarrow> t' < t" using True lastAcceptedTerm_Some_currentTerm unfolding nd_def by fastforce
-  qed
+  qed auto
 qed
 
 lemma (in zenStep) addElectionVote_invariants:
@@ -1097,8 +1123,8 @@ lemma (in zenStep) addElectionVote_invariants:
     "i < firstUncommittedSlot nd
         \<or> (i = firstUncommittedSlot nd
             \<and> (a = None
-                \<or> a = lastAcceptedTerm nd
-                \<or> (maxTermOption a (lastAcceptedTerm nd) = lastAcceptedTerm nd
+                \<or> a = lastAcceptedTermInSlot nd
+                \<or> (maxTermOption a (lastAcceptedTermInSlot nd) = lastAcceptedTermInSlot nd
                       \<and> electionValueForced nd)))"
   shows "zen messages' nodeState'"
 proof -
@@ -1117,13 +1143,15 @@ proof -
     "\<And>n. firstUncommittedSlot (nodeState' n) = firstUncommittedSlot (nodeState n)"
     "\<And>n. currentVotingNodes (nodeState' n) = currentVotingNodes (nodeState n)"
     "\<And>n q. isQuorum (nodeState' n) q = isQuorum (nodeState n) q"
+    "\<And>n. lastAcceptedSlot (nodeState' n) = lastAcceptedSlot (nodeState n)"
     "\<And>n. lastAcceptedTerm (nodeState' n) = lastAcceptedTerm (nodeState n)"
     "\<And>n. lastAcceptedValue (nodeState' n) = lastAcceptedValue (nodeState n)"
+    "\<And>n. lastAcceptedTermInSlot (nodeState' n) = lastAcceptedTermInSlot (nodeState n)"
     "\<And>n. currentTerm (nodeState' n) = currentTerm (nodeState n)"
     "\<And>n. publishPermitted (nodeState' n) = publishPermitted (nodeState n)"
     "\<And>n. publishVotes (nodeState' n) = publishVotes (nodeState n)"
     "\<And>n. currentClusterState (nodeState' n) = currentClusterState (nodeState n)"
-    by (unfold nodeState'_def, auto simp add: nd_def isQuorum_def nd' addElectionVote_def Let_def)
+    by (unfold nodeState'_def, auto simp add: nd_def isQuorum_def nd' addElectionVote_def Let_def lastAcceptedTermInSlot_def)
 
   have updated_properties:
     "\<And>n. joinVotes (nodeState' n) = joinVotes (nodeState n) \<union> (if n = n\<^sub>0 then {s} else {})"
@@ -1155,10 +1183,11 @@ proof -
     from JoinRequest_unique_destination show "\<And>i' i s t a a' d d'. s \<midarrow>\<langle> JoinRequest i t a \<rangle>\<rightarrow> d \<Longrightarrow> s \<midarrow>\<langle> JoinRequest i' t a' \<rangle>\<rightarrow> d' \<Longrightarrow> d = d'".
     from currentNode_nodeState show "\<And>n. currentNode (nodeState n) = n" .
     from committedTo_firstUncommittedSlot show "\<And>n. committed\<^sub>< (firstUncommittedSlot (nodeState n))" .
-    from firstUncommittedSlot_PublishResponse show "\<And>n i t. firstUncommittedSlot (nodeState n) < i \<Longrightarrow> \<not> n \<midarrow>\<langle> PublishResponse i t \<rangle>\<leadsto>" .
-    from lastAcceptedTerm_None show "\<And>n t. lastAcceptedTerm (nodeState n) = None \<Longrightarrow> \<not> n \<midarrow>\<langle> PublishResponse (firstUncommittedSlot (nodeState n)) t \<rangle>\<leadsto>".
-    from lastAcceptedTerm_Some_sent show "\<And>n t. lastAcceptedTerm (nodeState n) = Some t \<Longrightarrow> n \<midarrow>\<langle> PublishResponse (firstUncommittedSlot (nodeState n)) t \<rangle>\<leadsto>".
-    from lastAcceptedTerm_Some_max show "\<And>n t t'. lastAcceptedTerm (nodeState n) = Some t \<Longrightarrow> n \<midarrow>\<langle> PublishResponse (firstUncommittedSlot (nodeState n)) t' \<rangle>\<leadsto> \<Longrightarrow> t' \<le> t".
+    from lastAcceptedSlot_firstUncommittedSlot  show "\<And>n. lastAcceptedSlot (nodeState n) \<le> firstUncommittedSlot (nodeState n)".
+    from lastAcceptedSlot_PublishResponse show "\<And>n i t. lastAcceptedSlot (nodeState n) < i \<Longrightarrow> \<not> n \<midarrow>\<langle> PublishResponse i t \<rangle>\<leadsto>" .
+    from lastAcceptedTerm_None show "\<And>n t. lastAcceptedTerm (nodeState n) = None \<Longrightarrow> \<not> n \<midarrow>\<langle> PublishResponse (lastAcceptedSlot (nodeState n)) t \<rangle>\<leadsto>".
+    from lastAcceptedTerm_Some_sent show "\<And>n t. lastAcceptedTerm (nodeState n) = Some t \<Longrightarrow> n \<midarrow>\<langle> PublishResponse (lastAcceptedSlot (nodeState n)) t \<rangle>\<leadsto>".
+    from lastAcceptedTerm_Some_max show "\<And>n t t'. lastAcceptedTerm (nodeState n) = Some t \<Longrightarrow> n \<midarrow>\<langle> PublishResponse (lastAcceptedSlot (nodeState n)) t' \<rangle>\<leadsto> \<Longrightarrow> t' \<le> t".
     from JoinRequest_currentTerm show "\<And>n i t a. n \<midarrow>\<langle> JoinRequest i t a \<rangle>\<leadsto> \<Longrightarrow> t \<le> currentTerm (nodeState n)".
     from JoinRequest_slot_function show "\<And>n i i' t a a'. n \<midarrow>\<langle> JoinRequest i t a \<rangle>\<leadsto> \<Longrightarrow> n \<midarrow>\<langle> JoinRequest i' t a' \<rangle>\<leadsto> \<Longrightarrow> i = i'".
     from publishVotes show "\<And>n n'. n' \<in> publishVotes (nodeState n) \<Longrightarrow> n' \<midarrow>\<langle> PublishResponse (firstUncommittedSlot (nodeState n)) (currentTerm (nodeState n)) \<rangle>\<leadsto>".
@@ -1170,7 +1199,7 @@ proof -
     from ApplyCommit_quorum show "\<And>i t. \<langle> ApplyCommit i t \<rangle>\<leadsto> \<Longrightarrow> \<exists>q\<in>majorities (V i). \<forall>s\<in>q. s \<midarrow>\<langle> PublishResponse i t \<rangle>\<leadsto>".
     from currentVotingNodes_firstUncommittedSlot show "\<And>n. currentVotingNodes (nodeState n) = V (firstUncommittedSlot (nodeState n))".
     from firstUncommittedSlot_PublishRequest show "\<And>i n t x. firstUncommittedSlot (nodeState n) < i \<Longrightarrow> \<not> n \<midarrow>\<langle> PublishRequest i t x \<rangle>\<leadsto>".
-    from lastAcceptedTerm_Some_value show "\<And>n t. lastAcceptedTerm (nodeState n) = Some t \<Longrightarrow> \<langle> PublishRequest (firstUncommittedSlot (nodeState n)) t (lastAcceptedValue (nodeState n)) \<rangle>\<leadsto>".
+    from lastAcceptedTerm_Some_value show "\<And>n t. lastAcceptedTerm (nodeState n) = Some t \<Longrightarrow> \<langle> PublishRequest (lastAcceptedSlot (nodeState n)) t (lastAcceptedValue (nodeState n)) \<rangle>\<leadsto>".
     from PublishRequest_currentTerm show "\<And>n t x. n \<midarrow>\<langle> PublishRequest (firstUncommittedSlot (nodeState n)) t x \<rangle>\<leadsto> \<Longrightarrow> t \<le> currentTerm (nodeState n)".
     from PublishRequest_publishPermitted_currentTerm show "\<And>n t x. n \<midarrow>\<langle> PublishRequest (firstUncommittedSlot (nodeState n)) t x \<rangle>\<leadsto> \<Longrightarrow> publishPermitted (nodeState n) \<Longrightarrow> t < currentTerm (nodeState n)".
     from PublishRequest_quorum show "\<And>i s t x. s \<midarrow>\<langle> PublishRequest i t x \<rangle>\<leadsto> \<Longrightarrow> \<exists>q\<in>majorities (V i). (\<forall>n\<in>q. promised i n s t) \<and> (prevAccepted i t q = {} \<or> v i t = v i (maxTerm (prevAccepted i t q)))".
@@ -1188,19 +1217,20 @@ proof -
     show "\<And>n'. \<not> electionValueForced (nodeState' n) \<Longrightarrow> n' \<in> joinVotes (nodeState' n) \<Longrightarrow> n' \<midarrow>\<langle> JoinRequest (firstUncommittedSlot (nodeState n)) (currentTerm (nodeState n)) None \<rangle>\<rightarrow> (OneNode n) \<or> (\<exists>i<firstUncommittedSlot (nodeState n). \<exists>a. n' \<midarrow>\<langle> JoinRequest i (currentTerm (nodeState n)) a \<rangle>\<rightarrow> (OneNode n))"
       using precondition sent unfolding updated_properties nd_def by (cases "n = n\<^sub>0", auto)
 
-    from electionValueForced_JoinRequest
-    show "electionValueForced (nodeState' n) \<Longrightarrow> \<not> (\<exists>x. \<langle> PublishRequest (firstUncommittedSlot (nodeState n)) (currentTerm (nodeState n)) x \<rangle>\<leadsto>) \<Longrightarrow> \<exists>n'\<in>joinVotes (nodeState' n). n' \<midarrow>\<langle> JoinRequest (firstUncommittedSlot (nodeState n)) (currentTerm (nodeState n)) (lastAcceptedTerm (nodeState n)) \<rangle>\<rightarrow> (OneNode n)"
-      using precondition sent unfolding updated_properties nd_def by (cases "n = n\<^sub>0", auto)
-
-    from electionValueForced_max nd_def
-    show "\<And>n' a'. electionValueForced (nodeState' n) \<Longrightarrow> \<not> (\<exists>x. \<langle> PublishRequest (firstUncommittedSlot (nodeState n)) (currentTerm (nodeState n)) x \<rangle>\<leadsto>) \<Longrightarrow> n' \<in> joinVotes (nodeState' n) \<Longrightarrow> n' \<midarrow>\<langle> JoinRequest (firstUncommittedSlot (nodeState n)) (currentTerm (nodeState n)) a' \<rangle>\<rightarrow> (OneNode n) \<Longrightarrow> maxTermOption a' (lastAcceptedTerm (nodeState n)) = lastAcceptedTerm (nodeState n)"
-      using precondition sent unfolding updated_properties nd_def apply (cases "n = n\<^sub>0", simp_all)
-      by (metis electionValueFree_JoinRequest isMessageFromTo_def maxTermOption_None_t maxTermOption_diagonal nat_neq_iff zen.JoinRequest_slot_function zenMessages.JoinRequest_value_function zenMessages_axioms zen_axioms)
-
     from joinVotes nd_def precondition sent
     show "\<And>n'. n' \<in> joinVotes (nodeState' n) \<Longrightarrow> promised (firstUncommittedSlot (nodeState n)) n' n (currentTerm (nodeState n))"
       using precondition sent unfolding updated_properties nd_def apply (cases "n = n\<^sub>0", simp_all)
       using nd_def promised_def slot by blast
+
+    from electionValueForced_JoinRequest
+    show "electionValueForced (nodeState' n) \<Longrightarrow> \<not> (\<exists>x. \<langle> PublishRequest (firstUncommittedSlot (nodeState n)) (currentTerm (nodeState n)) x \<rangle>\<leadsto>) \<Longrightarrow> \<exists>n'\<in>joinVotes (nodeState' n). n' \<midarrow>\<langle> JoinRequest (firstUncommittedSlot (nodeState n)) (currentTerm (nodeState n)) (lastAcceptedTermInSlot (nodeState n)) \<rangle>\<rightarrow> (OneNode n)"
+      using precondition sent unfolding updated_properties nd_def by (cases "n = n\<^sub>0", auto)
+
+    from electionValueForced_max nd_def
+    show "\<And>n' a'. electionValueForced (nodeState' n) \<Longrightarrow> \<not> (\<exists>x. \<langle> PublishRequest (firstUncommittedSlot (nodeState n)) (currentTerm (nodeState n)) x \<rangle>\<leadsto>) \<Longrightarrow> n' \<in> joinVotes (nodeState' n) \<Longrightarrow> n' \<midarrow>\<langle> JoinRequest (firstUncommittedSlot (nodeState n)) (currentTerm (nodeState n)) a' \<rangle>\<rightarrow> (OneNode n) \<Longrightarrow> maxTermOption a' (lastAcceptedTermInSlot (nodeState n)) = lastAcceptedTermInSlot (nodeState n)"
+      using precondition sent unfolding updated_properties nd_def apply (cases "n = n\<^sub>0", simp_all)
+      by (metis electionValueFree_JoinRequest isMessageFromTo_def maxTermOption_None_t maxTermOption_diagonal nat_neq_iff zen.JoinRequest_slot_function zenMessages.JoinRequest_value_function zenMessages_axioms zen_axioms)
+
   qed
 qed
 
@@ -1399,15 +1429,17 @@ next
     "\<And>n. firstUncommittedSlot (nodeState' n) = firstUncommittedSlot (nodeState n)"
     "\<And>n. currentVotingNodes (nodeState' n) = currentVotingNodes (nodeState n)"
     "\<And>n q. isQuorum (nodeState' n) q = isQuorum (nodeState n) q"
+    "\<And>n. lastAcceptedSlot (nodeState' n) = lastAcceptedSlot (nodeState n)"
     "\<And>n. lastAcceptedTerm (nodeState' n) = lastAcceptedTerm (nodeState n)"
     "\<And>n. lastAcceptedValue (nodeState' n) = lastAcceptedValue (nodeState n)"
+    "\<And>n. lastAcceptedTermInSlot (nodeState' n) = lastAcceptedTermInSlot (nodeState n)"
     "\<And>n. currentTerm (nodeState' n) = currentTerm (nodeState n)"
     "\<And>n. publishVotes (nodeState' n) = publishVotes (nodeState n)"
     "\<And>n. currentClusterState (nodeState' n) = currentClusterState (nodeState n)"
     "\<And>n. electionWon (nodeState' n) = electionWon (nodeState n)"
     "\<And>n. joinVotes (nodeState' n) = joinVotes (nodeState n)"
     "\<And>n. electionValueForced (nodeState' n) = electionValueForced (nodeState n)"
-    by (unfold nodeState'_def, auto simp add: nd_def isQuorum_def nd' addElectionVote_def Let_def)
+    by (unfold nodeState'_def, auto simp add: nd_def isQuorum_def nd' addElectionVote_def Let_def lastAcceptedTermInSlot_def)
 
   show ?thesis
     apply (intro zenI)
@@ -1423,10 +1455,11 @@ next
     from JoinRequest_unique_destination show "\<And>i' i s t a a' d d'. s \<midarrow>\<langle> JoinRequest i t a \<rangle>\<rightarrow> d \<Longrightarrow> s \<midarrow>\<langle> JoinRequest i' t a' \<rangle>\<rightarrow> d' \<Longrightarrow> d = d'".
     from currentNode_nodeState show "\<And>n. currentNode (nodeState n) = n" .
     from committedTo_firstUncommittedSlot show "\<And>n. committed\<^sub>< (firstUncommittedSlot (nodeState n))" .
-    from firstUncommittedSlot_PublishResponse show "\<And>n i t. firstUncommittedSlot (nodeState n) < i \<Longrightarrow> \<not> n \<midarrow>\<langle> PublishResponse i t \<rangle>\<leadsto>" .
-    from lastAcceptedTerm_None show "\<And>n t. lastAcceptedTerm (nodeState n) = None \<Longrightarrow> \<not> n \<midarrow>\<langle> PublishResponse (firstUncommittedSlot (nodeState n)) t \<rangle>\<leadsto>".
-    from lastAcceptedTerm_Some_sent show "\<And>n t. lastAcceptedTerm (nodeState n) = Some t \<Longrightarrow> n \<midarrow>\<langle> PublishResponse (firstUncommittedSlot (nodeState n)) t \<rangle>\<leadsto>".
-    from lastAcceptedTerm_Some_max show "\<And>n t t'. lastAcceptedTerm (nodeState n) = Some t \<Longrightarrow> n \<midarrow>\<langle> PublishResponse (firstUncommittedSlot (nodeState n)) t' \<rangle>\<leadsto> \<Longrightarrow> t' \<le> t".
+    from lastAcceptedSlot_firstUncommittedSlot  show "\<And>n. lastAcceptedSlot (nodeState n) \<le> firstUncommittedSlot (nodeState n)".
+    from lastAcceptedSlot_PublishResponse show "\<And>n i t. lastAcceptedSlot (nodeState n) < i \<Longrightarrow> \<not> n \<midarrow>\<langle> PublishResponse i t \<rangle>\<leadsto>" .
+    from lastAcceptedTerm_None show "\<And>n t. lastAcceptedTerm (nodeState n) = None \<Longrightarrow> \<not> n \<midarrow>\<langle> PublishResponse (lastAcceptedSlot (nodeState n)) t \<rangle>\<leadsto>".
+    from lastAcceptedTerm_Some_sent show "\<And>n t. lastAcceptedTerm (nodeState n) = Some t \<Longrightarrow> n \<midarrow>\<langle> PublishResponse (lastAcceptedSlot (nodeState n)) t \<rangle>\<leadsto>".
+    from lastAcceptedTerm_Some_max show "\<And>n t t'. lastAcceptedTerm (nodeState n) = Some t \<Longrightarrow> n \<midarrow>\<langle> PublishResponse (lastAcceptedSlot (nodeState n)) t' \<rangle>\<leadsto> \<Longrightarrow> t' \<le> t".
     from JoinRequest_currentTerm show "\<And>n i t a. n \<midarrow>\<langle> JoinRequest i t a \<rangle>\<leadsto> \<Longrightarrow> t \<le> currentTerm (nodeState n)".
     from JoinRequest_slot_function show "\<And>n i i' t a a'. n \<midarrow>\<langle> JoinRequest i t a \<rangle>\<leadsto> \<Longrightarrow> n \<midarrow>\<langle> JoinRequest i' t a' \<rangle>\<leadsto> \<Longrightarrow> i = i'".
     from electionWon_isQuorum show "\<And>n. electionWon (nodeState n) \<Longrightarrow> isQuorum (nodeState n) (joinVotes (nodeState n))".
@@ -1446,7 +1479,7 @@ next
     }
 
     from lastAcceptedTerm_Some_value  PublishRequest'
-    show "\<And>n t. lastAcceptedTerm (nodeState n) = Some t \<Longrightarrow> \<langle> PublishRequest (firstUncommittedSlot (nodeState n)) t (lastAcceptedValue (nodeState n)) \<rangle>\<leadsto>'"
+    show "\<And>n t. lastAcceptedTerm (nodeState n) = Some t \<Longrightarrow> \<langle> PublishRequest (lastAcceptedSlot (nodeState n)) t (lastAcceptedValue (nodeState n)) \<rangle>\<leadsto>'"
       by (meson isMessage'_def isMessageFrom'_def isMessageFrom_def isMessage_def)
 
     from PublishRequest_currentTerm
@@ -1482,11 +1515,11 @@ next
       by (auto simp add: committedTo_def PublishRequest' nd_def)
 
     from electionValueForced_JoinRequest
-    show "electionValueForced (nodeState n) \<Longrightarrow> \<not> (\<exists>x. \<langle> PublishRequest (firstUncommittedSlot (nodeState n)) (currentTerm (nodeState n)) x \<rangle>\<leadsto>') \<Longrightarrow> \<exists>n'\<in>joinVotes (nodeState n). n' \<midarrow>\<langle> JoinRequest (firstUncommittedSlot (nodeState n)) (currentTerm (nodeState n)) (lastAcceptedTerm (nodeState n)) \<rangle>\<rightarrow> (OneNode n)"
+    show "electionValueForced (nodeState n) \<Longrightarrow> \<not> (\<exists>x. \<langle> PublishRequest (firstUncommittedSlot (nodeState n)) (currentTerm (nodeState n)) x \<rangle>\<leadsto>') \<Longrightarrow> \<exists>n'\<in>joinVotes (nodeState n). n' \<midarrow>\<langle> JoinRequest (firstUncommittedSlot (nodeState n)) (currentTerm (nodeState n)) (lastAcceptedTermInSlot (nodeState n)) \<rangle>\<rightarrow> (OneNode n)"
       by (cases "n = n\<^sub>0", simp_all add: nodeState'_def nd' PublishRequest')
 
     from electionValueForced_max
-    show "\<And>n' a'. electionValueForced (nodeState n) \<Longrightarrow> \<not> (\<exists>x. \<langle> PublishRequest (firstUncommittedSlot (nodeState n)) (currentTerm (nodeState n)) x \<rangle>\<leadsto>') \<Longrightarrow> n' \<in> joinVotes (nodeState n) \<Longrightarrow> n' \<midarrow>\<langle> JoinRequest (firstUncommittedSlot (nodeState n)) (currentTerm (nodeState n)) a' \<rangle>\<rightarrow> (OneNode n) \<Longrightarrow> maxTermOption a' (lastAcceptedTerm (nodeState n)) = lastAcceptedTerm (nodeState n)"
+    show "\<And>n' a'. electionValueForced (nodeState n) \<Longrightarrow> \<not> (\<exists>x. \<langle> PublishRequest (firstUncommittedSlot (nodeState n)) (currentTerm (nodeState n)) x \<rangle>\<leadsto>') \<Longrightarrow> n' \<in> joinVotes (nodeState n) \<Longrightarrow> n' \<midarrow>\<langle> JoinRequest (firstUncommittedSlot (nodeState n)) (currentTerm (nodeState n)) a' \<rangle>\<rightarrow> (OneNode n) \<Longrightarrow> maxTermOption a' (lastAcceptedTermInSlot (nodeState n)) = lastAcceptedTermInSlot (nodeState n)"
       by (cases "n = n\<^sub>0", auto simp add: nodeState'_def nd' PublishRequest')
 
     {
@@ -1568,7 +1601,7 @@ next
             qed
 
             from electionValueForced_nd electionValueForced_JoinRequest won
-            obtain n'' where n''_vote: "n'' \<in> q" and n''_sent: "n'' \<midarrow>\<langle> JoinRequest i t (lastAcceptedTerm nd) \<rangle>\<rightarrow> (OneNode n\<^sub>0)"
+            obtain n'' where n''_vote: "n'' \<in> q" and n''_sent: "n'' \<midarrow>\<langle> JoinRequest i t (lastAcceptedTermInSlot nd) \<rangle>\<rightarrow> (OneNode n\<^sub>0)"
               using \<open>i = firstUncommittedSlot nd\<close> \<open>t = currentTerm nd\<close> fresh_request nd_def q_def by blast
 
             have 2: "v' i t = x"
@@ -1587,8 +1620,8 @@ next
               show "\<langle> PublishRequest i (maxTerm (prevAccepted i t q)) (v i (maxTerm (prevAccepted i t q))) \<rangle>\<leadsto>"
                 by (intro JoinRequest_PublishRequest_v, auto simp add: isMessage_def isMessageFrom_def)
 
-              have "lastAcceptedTerm nd = Some (maxTerm (prevAccepted i t q))"
-              proof (cases "lastAcceptedTerm nd")
+              have "lastAcceptedTermInSlot nd = Some (maxTerm (prevAccepted i t q))"
+              proof (cases "lastAcceptedTermInSlot nd")
                 case None show ?thesis
                   using None electionValueForced_max electionValueForced_nd n'_sent n'_vote nd_def q_def won
                   using fresh_request by fastforce
@@ -1600,7 +1633,7 @@ next
                   by (intro maxTerm_max finite_prevAccepted, auto simp add: prevAccepted_def isMessageFrom_def)
 
                 moreover from n'_vote n'_sent electionValueForced_nd won
-                have "maxTermOption (Some (maxTerm (prevAccepted i t q))) (lastAcceptedTerm nd) = lastAcceptedTerm nd"
+                have "maxTermOption (Some (maxTerm (prevAccepted i t q))) (lastAcceptedTermInSlot nd) = lastAcceptedTermInSlot nd"
                   unfolding nd_def q_def using fresh_request
                   by (intro electionValueForced_max [where n' = n'], simp_all add: nd_def)
                 hence "maxTerm (prevAccepted i t q) \<le> t'"
@@ -1608,8 +1641,10 @@ next
 
                 ultimately show ?thesis by simp
               qed
-              with lastAcceptedTerm_Some_value
+              with lastAcceptedTerm_Some_value [of n\<^sub>0]
               show "\<langle> PublishRequest i (maxTerm (prevAccepted i t q)) (lastAcceptedValue nd) \<rangle>\<leadsto>"
+                unfolding nd_def lastAcceptedTermInSlot_def
+                apply (cases "firstUncommittedSlot (nodeState n\<^sub>0) = lastAcceptedSlot (nodeState n\<^sub>0)")
                 by (auto simp add: nd_def)
             qed
 
@@ -1635,8 +1670,8 @@ proof (cases "t = currentTerm nd
              \<and> (i < firstUncommittedSlot nd
                 \<or> (i = firstUncommittedSlot nd
                     \<and> (a = None
-                        \<or> a = lastAcceptedTerm nd
-                        \<or> (maxTermOption a (lastAcceptedTerm nd) = lastAcceptedTerm nd
+                        \<or> a = lastAcceptedTermInSlot nd
+                        \<or> (maxTermOption a (lastAcceptedTermInSlot nd) = lastAcceptedTermInSlot nd
                               \<and> electionValueForced nd))))")
   case False
   have [simp]: "result = (nd, None)" unfolding result_def handleJoinRequest_def by (simp add: False Let_def)
@@ -1647,7 +1682,7 @@ next
   case True
   hence True': "i \<le> firstUncommittedSlot nd"
     "t = currentTerm nd"
-    "i < firstUncommittedSlot nd \<or> (i = firstUncommittedSlot nd \<and> (a = None \<or> a = lastAcceptedTerm nd \<or> (maxTermOption a (lastAcceptedTerm nd) = lastAcceptedTerm nd \<and> electionValueForced nd)))"
+    "i < firstUncommittedSlot nd \<or> (i = firstUncommittedSlot nd \<and> (a = None \<or> a = lastAcceptedTermInSlot nd \<or> (maxTermOption a (lastAcceptedTermInSlot nd) = lastAcceptedTermInSlot nd \<and> electionValueForced nd)))"
     by auto
 
   define nd1 where "nd1 \<equiv> addElectionVote s i a nd"
@@ -1665,7 +1700,7 @@ next
       fold nd_def isMessageFromTo_def)
     show "nodeState1 n\<^sub>0 = addElectionVote s i a nd" by (simp add: nodeState1_def nd1_def)
     from True' sent show "s \<midarrow>\<langle> JoinRequest i (currentTerm nd) a \<rangle>\<rightarrow> (OneNode n\<^sub>0)" by simp
-    from True' show "i < firstUncommittedSlot nd \<or> i = firstUncommittedSlot nd \<and> (a = None \<or> a = lastAcceptedTerm nd \<or> maxTermOption a (lastAcceptedTerm nd) = lastAcceptedTerm nd \<and> electionValueForced nd)" by simp
+    from True' show "i < firstUncommittedSlot nd \<or> i = firstUncommittedSlot nd \<and> (a = None \<or> a = lastAcceptedTermInSlot nd \<or> maxTermOption a (lastAcceptedTermInSlot nd) = lastAcceptedTermInSlot nd \<and> electionValueForced nd)" by simp
     show "\<And>n. n \<noteq> n\<^sub>0 \<Longrightarrow> nodeState1 n = nodeState' n" unfolding nodeState1_def nodeState'_def by simp
   qed
 
@@ -1736,7 +1771,7 @@ proof (cases "i = firstUncommittedSlot nd \<and> t = currentTerm nd")
 next
   case precondition: True
 
-  hence result: "result = (nd\<lparr>lastAcceptedTerm := Some t, lastAcceptedValue := x\<rparr>,
+  hence result: "result = (nd\<lparr>lastAcceptedSlot := i, lastAcceptedTerm := Some t, lastAcceptedValue := x\<rparr>,
       Some (PublishResponse i t))"
     by (auto simp add: result_def handlePublishRequest_def)
 
@@ -1777,7 +1812,10 @@ next
     "\<And>n. electionValueForced (nodeState' n) = electionValueForced (nodeState n)"
     "lastAcceptedTerm nd' = Some t"
     "lastAcceptedValue nd' = x"
-    by (unfold nodeState'_def, auto simp add: result nd' nd_def isQuorum_def)
+    "lastAcceptedSlot nd' = i"
+    "lastAcceptedTermInSlot nd' = Some t"
+    using precondition
+    by (unfold nodeState'_def, auto simp add: result nd' nd_def isQuorum_def lastAcceptedTermInSlot_def)
 
   have updated_properties:
     "\<And>n. lastAcceptedTerm (nodeState' n) = (if n = n\<^sub>0 then Some t else lastAcceptedTerm (nodeState n))"
@@ -1846,26 +1884,34 @@ next
     from JoinRequest_Some_max show "\<And>i s t t' t''. s \<midarrow>\<langle> JoinRequest i t (Some t') \<rangle>\<leadsto> \<Longrightarrow> t' < t'' \<Longrightarrow> t'' < t \<Longrightarrow> \<not> s \<midarrow>\<langle> PublishResponse i t'' \<rangle>\<leadsto>'"
       using precondition unfolding PublishResponse' nd_def using JoinRequest_currentTerm by fastforce
 
-    from firstUncommittedSlot_PublishResponse show "\<And>n i t. firstUncommittedSlot (nodeState n) < i \<Longrightarrow> \<not> n \<midarrow>\<langle> PublishResponse i t \<rangle>\<leadsto>'"
-      using precondition unfolding PublishResponse' nd_def by blast
+    from lastAcceptedSlot_firstUncommittedSlot  show "\<And>n. lastAcceptedSlot (nodeState' n) \<le> firstUncommittedSlot (nodeState n)"
+      using precondition unfolding nd_def nodeState'_def by auto
 
-    from lastAcceptedTerm_None show "\<And>n t. lastAcceptedTerm (nodeState' n) = None \<Longrightarrow> \<not> n \<midarrow>\<langle> PublishResponse (firstUncommittedSlot (nodeState n)) t \<rangle>\<leadsto>'"
+    fix n
+
+    from lastAcceptedSlot_PublishResponse show "\<And>i t. lastAcceptedSlot (nodeState' n) < i \<Longrightarrow> \<not> n \<midarrow>\<langle> PublishResponse i t \<rangle>\<leadsto>'"
+      using precondition unfolding PublishResponse' nd_def nodeState'_def apply (cases "n = n\<^sub>0", auto)
+      by (meson dual_order.strict_trans1 leD lessI not_less_eq_eq lastAcceptedSlot_firstUncommittedSlot)
+
+    from lastAcceptedTerm_None show "\<And>n t. lastAcceptedTerm (nodeState' n) = None \<Longrightarrow> \<not> n \<midarrow>\<langle> PublishResponse (lastAcceptedSlot (nodeState' n)) t \<rangle>\<leadsto>'"
       using precondition property_simps unfolding PublishResponse' nd_def
       by (metis fst_conv nd'_def nodeState_unchanged option.distinct(1))
 
-    from lastAcceptedTerm_Some_sent show "\<And>n t. lastAcceptedTerm (nodeState' n) = Some t \<Longrightarrow> n \<midarrow>\<langle> PublishResponse (firstUncommittedSlot (nodeState n)) t \<rangle>\<leadsto>'"
+    from lastAcceptedTerm_Some_sent show "\<And>n t. lastAcceptedTerm (nodeState' n) = Some t \<Longrightarrow> n \<midarrow>\<langle> PublishResponse (lastAcceptedSlot (nodeState' n)) t \<rangle>\<leadsto>'"
       using precondition property_simps unfolding PublishResponse' nd_def
       by (metis nd'_def nodeState_unchanged option.inject)
 
-    from lastAcceptedTerm_Some_max show "\<And>n t t'. lastAcceptedTerm (nodeState' n) = Some t \<Longrightarrow> n \<midarrow>\<langle> PublishResponse (firstUncommittedSlot (nodeState n)) t' \<rangle>\<leadsto>' \<Longrightarrow> t' \<le> t"
-      using precondition property_simps unfolding PublishResponse' nd_def
-      by (metis Pair_inject dual_order.trans lastAcceptedTerm_None lastAcceptedTerm_Some_currentTerm nd'_def nodeState_unchanged not_None_eq option.inject order_refl)
+    from lastAcceptedTerm_Some_max show "\<And>t t'. lastAcceptedTerm (nodeState' n) = Some t \<Longrightarrow> n \<midarrow>\<langle> PublishResponse (lastAcceptedSlot (nodeState' n)) t' \<rangle>\<leadsto>' \<Longrightarrow> t' \<le> t"
+      using precondition property_simps unfolding PublishResponse' nd_def apply (cases "n = n\<^sub>0", auto)
+      apply (metis dual_order.trans lastAcceptedSlot_PublishResponse lastAcceptedSlot_firstUncommittedSlot lastAcceptedTerm_None lastAcceptedTerm_Some_currentTerm nat_less_le nd'_def not_Some_eq option.inject property_simps(12) property_simps(14))
+      using nd'_def property_simps apply auto
+      using nodeState_unchanged by auto
 
-    from electionValueForced_JoinRequest show "\<And>n. electionValueForced (nodeState n) \<Longrightarrow> \<not> (\<exists>x. \<langle> PublishRequest (firstUncommittedSlot (nodeState n)) (currentTerm (nodeState n)) x \<rangle>\<leadsto>) \<Longrightarrow> \<exists>n'\<in>joinVotes (nodeState n). n' \<midarrow>\<langle> JoinRequest (firstUncommittedSlot (nodeState n)) (currentTerm (nodeState n)) (lastAcceptedTerm (nodeState' n)) \<rangle>\<rightarrow> (OneNode n)"
+    from electionValueForced_JoinRequest show "\<And>n. electionValueForced (nodeState n) \<Longrightarrow> \<not> (\<exists>x. \<langle> PublishRequest (firstUncommittedSlot (nodeState n)) (currentTerm (nodeState n)) x \<rangle>\<leadsto>) \<Longrightarrow> \<exists>n'\<in>joinVotes (nodeState n). n' \<midarrow>\<langle> JoinRequest (firstUncommittedSlot (nodeState n)) (currentTerm (nodeState n)) (lastAcceptedTermInSlot (nodeState' n)) \<rangle>\<rightarrow> (OneNode n)"
       using precondition property_simps unfolding PublishResponse' nd_def
       by (metis isMessage_def nodeState_unchanged sent)
 
-    from electionValueForced_max show " \<And>n n' a'. electionValueForced (nodeState n) \<Longrightarrow> \<not> (\<exists>x. \<langle> PublishRequest (firstUncommittedSlot (nodeState n)) (currentTerm (nodeState n)) x \<rangle>\<leadsto>) \<Longrightarrow> n' \<in> joinVotes (nodeState n) \<Longrightarrow> n' \<midarrow>\<langle> JoinRequest (firstUncommittedSlot (nodeState n)) (currentTerm (nodeState n)) a' \<rangle>\<rightarrow> (OneNode n) \<Longrightarrow> maxTermOption a' (lastAcceptedTerm (nodeState' n)) = lastAcceptedTerm (nodeState' n)"
+    from electionValueForced_max show " \<And>n n' a'. electionValueForced (nodeState n) \<Longrightarrow> \<not> (\<exists>x. \<langle> PublishRequest (firstUncommittedSlot (nodeState n)) (currentTerm (nodeState n)) x \<rangle>\<leadsto>) \<Longrightarrow> n' \<in> joinVotes (nodeState n) \<Longrightarrow> n' \<midarrow>\<langle> JoinRequest (firstUncommittedSlot (nodeState n)) (currentTerm (nodeState n)) a' \<rangle>\<rightarrow> (OneNode n) \<Longrightarrow> maxTermOption a' (lastAcceptedTermInSlot (nodeState' n)) = lastAcceptedTermInSlot (nodeState' n)"
       using precondition property_simps unfolding PublishResponse' nd_def
       by (metis isMessage_def nodeState_unchanged sent)
 
@@ -1881,7 +1927,7 @@ next
       using precondition property_simps unfolding PublishResponse' nd_def
       by meson
 
-    from lastAcceptedTerm_Some_value show "\<And>n t. lastAcceptedTerm (nodeState' n) = Some t \<Longrightarrow> \<langle> PublishRequest (firstUncommittedSlot (nodeState n)) t (lastAcceptedValue (nodeState' n)) \<rangle>\<leadsto>"
+    from lastAcceptedTerm_Some_value show "\<And>n t. lastAcceptedTerm (nodeState' n) = Some t \<Longrightarrow> \<langle> PublishRequest (lastAcceptedSlot (nodeState' n)) t (lastAcceptedValue (nodeState' n)) \<rangle>\<leadsto>"
       using precondition property_simps unfolding PublishResponse' nd_def
       by (metis isMessage_def nd'_def nodeState_unchanged option.inject sent)
 
@@ -1913,13 +1959,15 @@ proof -
     "\<And>n q. isQuorum (nodeState' n) q = isQuorum (nodeState n) q"
     "\<And>n. lastAcceptedTerm (nodeState' n) = lastAcceptedTerm (nodeState n)"
     "\<And>n. lastAcceptedValue (nodeState' n) = lastAcceptedValue (nodeState n)"
+    "\<And>n. lastAcceptedSlot (nodeState' n) = lastAcceptedSlot (nodeState n)"
+    "\<And>n. lastAcceptedTermInSlot (nodeState' n) = lastAcceptedTermInSlot (nodeState n)"
     "\<And>n. currentTerm (nodeState' n) = currentTerm (nodeState n)"
     "\<And>n. publishPermitted (nodeState' n) = publishPermitted (nodeState n)"
     "\<And>n. joinVotes (nodeState' n) = joinVotes (nodeState n)"
     "\<And>n. electionWon (nodeState' n) = electionWon (nodeState n)"
     "\<And>n. electionValueForced (nodeState' n) = electionValueForced (nodeState n)"
    "\<And>n. currentClusterState (nodeState' n) = currentClusterState (nodeState n)"
-    by (unfold nodeState'_def, auto simp add: nd_def isQuorum_def nd' addElectionVote_def Let_def)
+    by (unfold nodeState'_def, auto simp add: nd_def isQuorum_def nd' addElectionVote_def Let_def lastAcceptedTermInSlot_def)
 
   have updated_properties[simp]:
     "\<And>n. publishVotes (nodeState' n) = publishVotes (nodeState n) \<union> (if n = n\<^sub>0 then {s} else {})"
@@ -1950,16 +1998,17 @@ proof -
     from JoinRequest_unique_destination show "\<And>i' i s t a a' d d'. s \<midarrow>\<langle> JoinRequest i t a \<rangle>\<rightarrow> d \<Longrightarrow> s \<midarrow>\<langle> JoinRequest i' t a' \<rangle>\<rightarrow> d' \<Longrightarrow> d = d'".
     from currentNode_nodeState show "\<And>n. currentNode (nodeState n) = n" .
     from committedTo_firstUncommittedSlot show "\<And>n. committed\<^sub>< (firstUncommittedSlot (nodeState n))" .
-    from firstUncommittedSlot_PublishResponse show "\<And>n i t. firstUncommittedSlot (nodeState n) < i \<Longrightarrow> \<not> n \<midarrow>\<langle> PublishResponse i t \<rangle>\<leadsto>" .
-    from lastAcceptedTerm_None show "\<And>n t. lastAcceptedTerm (nodeState n) = None \<Longrightarrow> \<not> n \<midarrow>\<langle> PublishResponse (firstUncommittedSlot (nodeState n)) t \<rangle>\<leadsto>".
-    from lastAcceptedTerm_Some_sent show "\<And>n t. lastAcceptedTerm (nodeState n) = Some t \<Longrightarrow> n \<midarrow>\<langle> PublishResponse (firstUncommittedSlot (nodeState n)) t \<rangle>\<leadsto>".
-    from lastAcceptedTerm_Some_max show "\<And>n t t'. lastAcceptedTerm (nodeState n) = Some t \<Longrightarrow> n \<midarrow>\<langle> PublishResponse (firstUncommittedSlot (nodeState n)) t' \<rangle>\<leadsto> \<Longrightarrow> t' \<le> t".
+    from lastAcceptedSlot_firstUncommittedSlot  show "\<And>n. lastAcceptedSlot (nodeState n) \<le> firstUncommittedSlot (nodeState n)".
+    from lastAcceptedSlot_PublishResponse show "\<And>n i t. lastAcceptedSlot (nodeState n) < i \<Longrightarrow> \<not> n \<midarrow>\<langle> PublishResponse i t \<rangle>\<leadsto>" .
+    from lastAcceptedTerm_None show "\<And>n t. lastAcceptedTerm (nodeState n) = None \<Longrightarrow> \<not> n \<midarrow>\<langle> PublishResponse (lastAcceptedSlot (nodeState n)) t \<rangle>\<leadsto>".
+    from lastAcceptedTerm_Some_sent show "\<And>n t. lastAcceptedTerm (nodeState n) = Some t \<Longrightarrow> n \<midarrow>\<langle> PublishResponse (lastAcceptedSlot (nodeState n)) t \<rangle>\<leadsto>".
+    from lastAcceptedTerm_Some_max show "\<And>n t t'. lastAcceptedTerm (nodeState n) = Some t \<Longrightarrow> n \<midarrow>\<langle> PublishResponse (lastAcceptedSlot (nodeState n)) t' \<rangle>\<leadsto> \<Longrightarrow> t' \<le> t".
     from JoinRequest_currentTerm show "\<And>n i t a. n \<midarrow>\<langle> JoinRequest i t a \<rangle>\<leadsto> \<Longrightarrow> t \<le> currentTerm (nodeState n)".
     from JoinRequest_slot_function show "\<And>n i i' t a a'. n \<midarrow>\<langle> JoinRequest i t a \<rangle>\<leadsto> \<Longrightarrow> n \<midarrow>\<langle> JoinRequest i' t a' \<rangle>\<leadsto> \<Longrightarrow> i = i'".
     from electionWon_isQuorum show "\<And>n. electionWon (nodeState n) \<Longrightarrow> isQuorum (nodeState n) (joinVotes (nodeState n))".
     from electionValueFree_JoinRequest show "\<And>n n'. \<not> electionValueForced (nodeState n) \<Longrightarrow> n' \<in> joinVotes (nodeState n) \<Longrightarrow> n' \<midarrow>\<langle> JoinRequest (firstUncommittedSlot (nodeState n)) (currentTerm (nodeState n)) None \<rangle>\<rightarrow> (OneNode n) \<or> (\<exists>i<firstUncommittedSlot (nodeState n). \<exists>a. n' \<midarrow>\<langle> JoinRequest i (currentTerm (nodeState n)) a \<rangle>\<rightarrow> (OneNode n))".
-    from electionValueForced_JoinRequest show "\<And>n. electionValueForced (nodeState n) \<Longrightarrow> \<not> (\<exists>x. \<langle> PublishRequest (firstUncommittedSlot (nodeState n)) (currentTerm (nodeState n)) x \<rangle>\<leadsto>) \<Longrightarrow> \<exists>n'\<in>joinVotes (nodeState n). n' \<midarrow>\<langle> JoinRequest (firstUncommittedSlot (nodeState n)) (currentTerm (nodeState n)) (lastAcceptedTerm (nodeState n)) \<rangle>\<rightarrow> (OneNode n)".
-    from electionValueForced_max show " \<And>n n' a'. electionValueForced (nodeState n) \<Longrightarrow> \<not> (\<exists>x. \<langle> PublishRequest (firstUncommittedSlot (nodeState n)) (currentTerm (nodeState n)) x \<rangle>\<leadsto>) \<Longrightarrow> n' \<in> joinVotes (nodeState n) \<Longrightarrow> n' \<midarrow>\<langle> JoinRequest (firstUncommittedSlot (nodeState n)) (currentTerm (nodeState n)) a' \<rangle>\<rightarrow> (OneNode n) \<Longrightarrow> maxTermOption a' (lastAcceptedTerm (nodeState n)) = lastAcceptedTerm (nodeState n)".
+    from electionValueForced_JoinRequest show "\<And>n. electionValueForced (nodeState n) \<Longrightarrow> \<not> (\<exists>x. \<langle> PublishRequest (firstUncommittedSlot (nodeState n)) (currentTerm (nodeState n)) x \<rangle>\<leadsto>) \<Longrightarrow> \<exists>n'\<in>joinVotes (nodeState n). n' \<midarrow>\<langle> JoinRequest (firstUncommittedSlot (nodeState n)) (currentTerm (nodeState n)) (lastAcceptedTermInSlot (nodeState n)) \<rangle>\<rightarrow> (OneNode n)".
+    from electionValueForced_max show " \<And>n n' a'. electionValueForced (nodeState n) \<Longrightarrow> \<not> (\<exists>x. \<langle> PublishRequest (firstUncommittedSlot (nodeState n)) (currentTerm (nodeState n)) x \<rangle>\<leadsto>) \<Longrightarrow> n' \<in> joinVotes (nodeState n) \<Longrightarrow> n' \<midarrow>\<langle> JoinRequest (firstUncommittedSlot (nodeState n)) (currentTerm (nodeState n)) a' \<rangle>\<rightarrow> (OneNode n) \<Longrightarrow> maxTermOption a' (lastAcceptedTermInSlot (nodeState n)) = lastAcceptedTermInSlot (nodeState n)".
     from currentClusterState_lastCommittedClusterStateBefore show "\<And>n. currentClusterState (nodeState n) = lastCommittedClusterStateBefore (firstUncommittedSlot (nodeState n))".
     from joinVotes show "\<And>n n'. n' \<in> joinVotes (nodeState n) \<Longrightarrow> promised (firstUncommittedSlot (nodeState n)) n' n (currentTerm (nodeState n))".
     from PublishRequest_committedTo show "\<And>i t x. \<langle> PublishRequest i t x \<rangle>\<leadsto> \<Longrightarrow> committed\<^sub>< i".
@@ -1969,7 +2018,7 @@ proof -
     from ApplyCommit_quorum show "\<And>i t. \<langle> ApplyCommit i t \<rangle>\<leadsto> \<Longrightarrow> \<exists>q\<in>majorities (V i). \<forall>s\<in>q. s \<midarrow>\<langle> PublishResponse i t \<rangle>\<leadsto>".
     from currentVotingNodes_firstUncommittedSlot show "\<And>n. currentVotingNodes (nodeState n) = V (firstUncommittedSlot (nodeState n))".
     from firstUncommittedSlot_PublishRequest show "\<And>i n t x. firstUncommittedSlot (nodeState n) < i \<Longrightarrow> \<not> n \<midarrow>\<langle> PublishRequest i t x \<rangle>\<leadsto>".
-    from lastAcceptedTerm_Some_value show "\<And>n t. lastAcceptedTerm (nodeState n) = Some t \<Longrightarrow> \<langle> PublishRequest (firstUncommittedSlot (nodeState n)) t (lastAcceptedValue (nodeState n)) \<rangle>\<leadsto>".
+    from lastAcceptedTerm_Some_value show "\<And>n t. lastAcceptedTerm (nodeState n) = Some t \<Longrightarrow> \<langle> PublishRequest (lastAcceptedSlot (nodeState n)) t (lastAcceptedValue (nodeState n)) \<rangle>\<leadsto>".
     from PublishRequest_currentTerm show "\<And>n t x. n \<midarrow>\<langle> PublishRequest (firstUncommittedSlot (nodeState n)) t x \<rangle>\<leadsto> \<Longrightarrow> t \<le> currentTerm (nodeState n)".
     from PublishRequest_publishPermitted_currentTerm show "\<And>n t x. n \<midarrow>\<langle> PublishRequest (firstUncommittedSlot (nodeState n)) t x \<rangle>\<leadsto> \<Longrightarrow> publishPermitted (nodeState n) \<Longrightarrow> t < currentTerm (nodeState n)".
      from CatchUpResponse_committedTo show "\<And>i conf cs. \<langle> CatchUpResponse i conf cs \<rangle>\<leadsto> \<Longrightarrow> committed\<^sub>< i".
@@ -2154,16 +2203,17 @@ next
     from JoinRequest_not_broadcast show "\<And>i t a d. \<langle> JoinRequest i t a \<rangle>\<rightarrow> d \<Longrightarrow> d \<noteq> Broadcast".
     from JoinRequest_unique_destination show "\<And>i' i s t a a' d d'. s \<midarrow>\<langle> JoinRequest i t a \<rangle>\<rightarrow> d \<Longrightarrow> s \<midarrow>\<langle> JoinRequest i' t a' \<rangle>\<rightarrow> d' \<Longrightarrow> d = d'".
     from currentNode_nodeState show "\<And>n. currentNode (nodeState n) = n" .
-    from firstUncommittedSlot_PublishResponse show "\<And>n i t. firstUncommittedSlot (nodeState n) < i \<Longrightarrow> \<not> n \<midarrow>\<langle> PublishResponse i t \<rangle>\<leadsto>" .
-    from lastAcceptedTerm_None show "\<And>n t. lastAcceptedTerm (nodeState n) = None \<Longrightarrow> \<not> n \<midarrow>\<langle> PublishResponse (firstUncommittedSlot (nodeState n)) t \<rangle>\<leadsto>".
-    from lastAcceptedTerm_Some_sent show "\<And>n t. lastAcceptedTerm (nodeState n) = Some t \<Longrightarrow> n \<midarrow>\<langle> PublishResponse (firstUncommittedSlot (nodeState n)) t \<rangle>\<leadsto>".
-    from lastAcceptedTerm_Some_max show "\<And>n t t'. lastAcceptedTerm (nodeState n) = Some t \<Longrightarrow> n \<midarrow>\<langle> PublishResponse (firstUncommittedSlot (nodeState n)) t' \<rangle>\<leadsto> \<Longrightarrow> t' \<le> t".
+    from lastAcceptedSlot_firstUncommittedSlot  show "\<And>n. lastAcceptedSlot (nodeState n) \<le> firstUncommittedSlot (nodeState n)".
+    from lastAcceptedSlot_PublishResponse show "\<And>n i t. lastAcceptedSlot (nodeState n) < i \<Longrightarrow> \<not> n \<midarrow>\<langle> PublishResponse i t \<rangle>\<leadsto>" .
+    from lastAcceptedTerm_None show "\<And>n t. lastAcceptedTerm (nodeState n) = None \<Longrightarrow> \<not> n \<midarrow>\<langle> PublishResponse (lastAcceptedSlot (nodeState n)) t \<rangle>\<leadsto>".
+    from lastAcceptedTerm_Some_sent show "\<And>n t. lastAcceptedTerm (nodeState n) = Some t \<Longrightarrow> n \<midarrow>\<langle> PublishResponse (lastAcceptedSlot (nodeState n)) t \<rangle>\<leadsto>".
+    from lastAcceptedTerm_Some_max show "\<And>n t t'. lastAcceptedTerm (nodeState n) = Some t \<Longrightarrow> n \<midarrow>\<langle> PublishResponse (lastAcceptedSlot (nodeState n)) t' \<rangle>\<leadsto> \<Longrightarrow> t' \<le> t".
     from JoinRequest_currentTerm show "\<And>n i t a. n \<midarrow>\<langle> JoinRequest i t a \<rangle>\<leadsto> \<Longrightarrow> t \<le> currentTerm (nodeState n)".
     from JoinRequest_slot_function show "\<And>n i i' t a a'. n \<midarrow>\<langle> JoinRequest i t a \<rangle>\<leadsto> \<Longrightarrow> n \<midarrow>\<langle> JoinRequest i' t a' \<rangle>\<leadsto> \<Longrightarrow> i = i'".
     from electionWon_isQuorum show "\<And>n. electionWon (nodeState n) \<Longrightarrow> isQuorum (nodeState n) (joinVotes (nodeState n))".
     from electionValueFree_JoinRequest show "\<And>n n'. \<not> electionValueForced (nodeState n) \<Longrightarrow> n' \<in> joinVotes (nodeState n) \<Longrightarrow> n' \<midarrow>\<langle> JoinRequest (firstUncommittedSlot (nodeState n)) (currentTerm (nodeState n)) None \<rangle>\<rightarrow> (OneNode n) \<or> (\<exists>i<firstUncommittedSlot (nodeState n). \<exists>a. n' \<midarrow>\<langle> JoinRequest i (currentTerm (nodeState n)) a \<rangle>\<rightarrow> (OneNode n))".
-    from electionValueForced_JoinRequest show "\<And>n. electionValueForced (nodeState n) \<Longrightarrow> \<not> (\<exists>x. \<langle> PublishRequest (firstUncommittedSlot (nodeState n)) (currentTerm (nodeState n)) x \<rangle>\<leadsto>) \<Longrightarrow> \<exists>n'\<in>joinVotes (nodeState n). n' \<midarrow>\<langle> JoinRequest (firstUncommittedSlot (nodeState n)) (currentTerm (nodeState n)) (lastAcceptedTerm (nodeState n)) \<rangle>\<rightarrow> (OneNode n)".
-    from electionValueForced_max show " \<And>n n' a'. electionValueForced (nodeState n) \<Longrightarrow> \<not> (\<exists>x. \<langle> PublishRequest (firstUncommittedSlot (nodeState n)) (currentTerm (nodeState n)) x \<rangle>\<leadsto>) \<Longrightarrow> n' \<in> joinVotes (nodeState n) \<Longrightarrow> n' \<midarrow>\<langle> JoinRequest (firstUncommittedSlot (nodeState n)) (currentTerm (nodeState n)) a' \<rangle>\<rightarrow> (OneNode n) \<Longrightarrow> maxTermOption a' (lastAcceptedTerm (nodeState n)) = lastAcceptedTerm (nodeState n)".
+    from electionValueForced_JoinRequest show "\<And>n. electionValueForced (nodeState n) \<Longrightarrow> \<not> (\<exists>x. \<langle> PublishRequest (firstUncommittedSlot (nodeState n)) (currentTerm (nodeState n)) x \<rangle>\<leadsto>) \<Longrightarrow> \<exists>n'\<in>joinVotes (nodeState n). n' \<midarrow>\<langle> JoinRequest (firstUncommittedSlot (nodeState n)) (currentTerm (nodeState n)) (lastAcceptedTermInSlot (nodeState n)) \<rangle>\<rightarrow> (OneNode n)".
+    from electionValueForced_max show " \<And>n n' a'. electionValueForced (nodeState n) \<Longrightarrow> \<not> (\<exists>x. \<langle> PublishRequest (firstUncommittedSlot (nodeState n)) (currentTerm (nodeState n)) x \<rangle>\<leadsto>) \<Longrightarrow> n' \<in> joinVotes (nodeState n) \<Longrightarrow> n' \<midarrow>\<langle> JoinRequest (firstUncommittedSlot (nodeState n)) (currentTerm (nodeState n)) a' \<rangle>\<rightarrow> (OneNode n) \<Longrightarrow> maxTermOption a' (lastAcceptedTermInSlot (nodeState n)) = lastAcceptedTermInSlot (nodeState n)".
     from publishVotes show "\<And>n n'. n' \<in> publishVotes (nodeState n) \<Longrightarrow> n' \<midarrow>\<langle> PublishResponse (firstUncommittedSlot (nodeState n)) (currentTerm (nodeState n)) \<rangle>\<leadsto>".
     from currentClusterState_lastCommittedClusterStateBefore show "\<And>n. currentClusterState (nodeState n) = lastCommittedClusterStateBefore (firstUncommittedSlot (nodeState n))".
     from joinVotes show "\<And>n n'. n' \<in> joinVotes (nodeState n) \<Longrightarrow> promised (firstUncommittedSlot (nodeState n)) n' n (currentTerm (nodeState n))".
@@ -2171,7 +2221,7 @@ next
     from PublishResponse_PublishRequest show "\<And>i s t. s \<midarrow>\<langle> PublishResponse i t \<rangle>\<leadsto> \<Longrightarrow> \<exists>x. \<langle> PublishRequest i t x \<rangle>\<leadsto>".
     from currentVotingNodes_firstUncommittedSlot show "\<And>n. currentVotingNodes (nodeState n) = V (firstUncommittedSlot (nodeState n))".
     from firstUncommittedSlot_PublishRequest show "\<And>i n t x. firstUncommittedSlot (nodeState n) < i \<Longrightarrow> \<not> n \<midarrow>\<langle> PublishRequest i t x \<rangle>\<leadsto>".
-    from lastAcceptedTerm_Some_value show "\<And>n t. lastAcceptedTerm (nodeState n) = Some t \<Longrightarrow> \<langle> PublishRequest (firstUncommittedSlot (nodeState n)) t (lastAcceptedValue (nodeState n)) \<rangle>\<leadsto>".
+    from lastAcceptedTerm_Some_value show "\<And>n t. lastAcceptedTerm (nodeState n) = Some t \<Longrightarrow> \<langle> PublishRequest (lastAcceptedSlot (nodeState n)) t (lastAcceptedValue (nodeState n)) \<rangle>\<leadsto>".
     from PublishRequest_currentTerm show "\<And>n t x. n \<midarrow>\<langle> PublishRequest (firstUncommittedSlot (nodeState n)) t x \<rangle>\<leadsto> \<Longrightarrow> t \<le> currentTerm (nodeState n)".
     from PublishRequest_publishPermitted_currentTerm show "\<And>n t x. n \<midarrow>\<langle> PublishRequest (firstUncommittedSlot (nodeState n)) t x \<rangle>\<leadsto> \<Longrightarrow> publishPermitted (nodeState n) \<Longrightarrow> t < currentTerm (nodeState n)".
     from lastAcceptedTerm_Some_currentTerm show "\<And>n t. lastAcceptedTerm (nodeState n) = Some t \<Longrightarrow> t \<le> currentTerm (nodeState n)".
@@ -2268,7 +2318,7 @@ lemma (in zenStep) handleApplyCommit_invariants:
   assumes messages'[simp]: "messages' = messages"
   assumes sent: "\<langle> ApplyCommit i t \<rangle>\<leadsto>"
  shows "zen messages' nodeState'"
-proof (cases "i = firstUncommittedSlot nd \<and> lastAcceptedTerm nd = Some t")
+proof (cases "i = firstUncommittedSlot nd \<and> lastAcceptedTermInSlot nd = Some t")
   case False
   hence nd'[simp]: "nd' = nd"
     by (auto simp add: nd' handleApplyCommit_def)
@@ -2280,7 +2330,13 @@ proof (cases "i = firstUncommittedSlot nd \<and> lastAcceptedTerm nd = Some t")
 next
   case True
   hence i: "i = firstUncommittedSlot nd"
-    and t: "lastAcceptedTerm nd = Some t" by simp_all
+    and t: "lastAcceptedTermInSlot nd = Some t" by simp_all
+
+  from t have "lastAcceptedSlot nd = firstUncommittedSlot nd \<and> lastAcceptedTerm nd = lastAcceptedTermInSlot nd"
+    unfolding lastAcceptedTermInSlot_def by (cases "firstUncommittedSlot nd = lastAcceptedSlot nd", auto)
+
+  hence lastAccepted_eqs[simp]: "lastAcceptedSlot (nodeState n\<^sub>0) = firstUncommittedSlot (nodeState n\<^sub>0)"
+    "lastAcceptedTerm (nodeState n\<^sub>0) = lastAcceptedTermInSlot (nodeState n\<^sub>0)" by (simp_all add: nd_def)
 
   have message_simps[simp]:
     "\<And>s p d. (s \<midarrow>\<langle> p \<rangle>\<rightarrow>' d) = (s \<midarrow>\<langle> p \<rangle>\<rightarrow> d)"
@@ -2302,8 +2358,8 @@ next
 
   from sent t
   have lastAcceptedValue_eq: "v\<^sub>c i = lastAcceptedValue nd"
-    unfolding i nd_def
-    by (intro PublishRequest_function [OF ApplyCommit_PublishRequest_v\<^sub>c lastAcceptedTerm_Some_value])
+    unfolding i nd_def using lastAcceptedTerm_Some_value [of n\<^sub>0 t]
+    by (intro PublishRequest_function [OF ApplyCommit_PublishRequest_v\<^sub>c], auto)
 
   show ?thesis
   proof (cases "isReconfiguration (v\<^sub>c i)")
@@ -2314,7 +2370,10 @@ next
       \<and> currentVotingNodes (nodeState' n) = currentVotingNodes (nodeState n)
       \<and> joinVotes (nodeState' n) = joinVotes (nodeState n)
       \<and> electionWon (nodeState' n) = electionWon (nodeState n)
-      \<and> isQuorum (nodeState' n) = isQuorum (nodeState n)"
+      \<and> isQuorum (nodeState' n) = isQuorum (nodeState n)
+      \<and> lastAcceptedTerm (nodeState' n) = lastAcceptedTerm (nodeState n)
+      \<and> lastAcceptedValue (nodeState' n) = lastAcceptedValue (nodeState n)
+      \<and> lastAcceptedSlot (nodeState' n) = lastAcceptedSlot (nodeState n)"
     proof (cases "v\<^sub>c i")
       case NoOp
       thus "\<And>n. ?thesis n"
@@ -2333,14 +2392,15 @@ next
       "\<And>n. joinVotes (nodeState' n) = joinVotes (nodeState n)"
       "\<And>n. electionWon (nodeState' n) = electionWon (nodeState n)"
       "\<And>n. isQuorum (nodeState' n) = isQuorum (nodeState n)"
+      "\<And>n. lastAcceptedTerm (nodeState' n) = lastAcceptedTerm (nodeState n)"
+      "\<And>n. lastAcceptedValue (nodeState' n) = lastAcceptedValue (nodeState n)"
+      "\<And>n. lastAcceptedSlot (nodeState' n) = lastAcceptedSlot (nodeState n)"
       by simp_all
 
     have "\<And>n. firstUncommittedSlot (nodeState' n) = (if n = n\<^sub>0 then Suc (firstUncommittedSlot (nodeState n)) else firstUncommittedSlot (nodeState n))
      \<and> publishPermitted (nodeState' n) = (publishPermitted (nodeState n) \<or> n = n\<^sub>0)
      \<and> publishVotes (nodeState' n) = (if n = n\<^sub>0 then {} else publishVotes (nodeState n))
-     \<and> electionValueForced (nodeState' n) = (electionValueForced (nodeState n) \<and> n \<noteq> n\<^sub>0)
-     \<and> lastAcceptedTerm (nodeState' n) = (if n = n\<^sub>0 then None else lastAcceptedTerm (nodeState n))
-     \<and> lastAcceptedValue (nodeState' n) = (if n = n\<^sub>0 then NoOp else lastAcceptedValue (nodeState n))"
+     \<and> electionValueForced (nodeState' n) = (electionValueForced (nodeState n) \<and> n \<noteq> n\<^sub>0)"
     proof (cases "v\<^sub>c i")
       case NoOp
       with i t show "\<And>n. ?thesis n"
@@ -2357,9 +2417,11 @@ next
       "\<And>n. publishPermitted (nodeState' n) = (publishPermitted (nodeState n) \<or> n = n\<^sub>0)"
       "\<And>n. publishVotes (nodeState' n) = (if n = n\<^sub>0 then {} else publishVotes (nodeState n))"
       "\<And>n. electionValueForced (nodeState' n) = (electionValueForced (nodeState n) \<and> n \<noteq> n\<^sub>0)"
-      "\<And>n. lastAcceptedTerm (nodeState' n) = (if n = n\<^sub>0 then None else lastAcceptedTerm (nodeState n))"
-      "\<And>n. lastAcceptedValue (nodeState' n) = (if n = n\<^sub>0 then NoOp else lastAcceptedValue (nodeState n))"
       by simp_all
+
+    have "\<And>n. lastAcceptedTermInSlot (nodeState' n) = (if n = n\<^sub>0 then None else lastAcceptedTermInSlot (nodeState n))"
+      unfolding lastAcceptedTermInSlot_def updated_properties property_simps by auto
+    note updated_properties = updated_properties this
 
     show ?thesis
       apply (intro zenI)
@@ -2386,6 +2448,12 @@ next
       from CatchUpResponse_committedTo show "\<And>i conf cs. \<langle> CatchUpResponse i conf cs \<rangle>\<leadsto> \<Longrightarrow> committed\<^sub>< i".
       from CatchUpResponse_V show "\<And>i conf cs. \<langle> CatchUpResponse i conf cs \<rangle>\<leadsto> \<Longrightarrow> V i = conf".
       from CatchUpResponse_lastCommittedClusterStateBefore show "\<And>i conf cs. \<langle> CatchUpResponse i conf cs \<rangle>\<leadsto> \<Longrightarrow> lastCommittedClusterStateBefore i = cs".
+      from lastAcceptedSlot_PublishResponse show "\<And>n i t. lastAcceptedSlot (nodeState n) < i \<Longrightarrow> \<not> n \<midarrow>\<langle> PublishResponse i t \<rangle>\<leadsto>".
+      from lastAcceptedTerm_None show "\<And>n t. lastAcceptedTerm (nodeState n) = None \<Longrightarrow> \<not> n \<midarrow>\<langle> PublishResponse (lastAcceptedSlot (nodeState n)) t \<rangle>\<leadsto>".
+      from lastAcceptedTerm_Some_sent show "\<And>n t. lastAcceptedTerm (nodeState n) = Some t \<Longrightarrow> n \<midarrow>\<langle> PublishResponse (lastAcceptedSlot (nodeState n)) t \<rangle>\<leadsto>".
+      from lastAcceptedTerm_Some_max show "\<And>n t t'. lastAcceptedTerm (nodeState n) = Some t \<Longrightarrow> n \<midarrow>\<langle> PublishResponse (lastAcceptedSlot (nodeState n)) t' \<rangle>\<leadsto> \<Longrightarrow> t' \<le> t".
+      from lastAcceptedTerm_Some_value show "\<And>n t. lastAcceptedTerm (nodeState n) = Some t \<Longrightarrow> \<langle> PublishRequest (lastAcceptedSlot (nodeState n)) t (lastAcceptedValue (nodeState n)) \<rangle>\<leadsto>".
+      from lastAcceptedTerm_Some_currentTerm show "\<And>n t. lastAcceptedTerm (nodeState n) = Some t \<Longrightarrow> t \<le> currentTerm (nodeState n)".
 
       fix n
 
@@ -2393,26 +2461,17 @@ next
         unfolding updated_properties committedTo_def apply (cases "n = n\<^sub>0", auto)
         using i isCommitted_def less_antisym nd_def sent by blast
 
-      from firstUncommittedSlot_PublishResponse show "\<And>i t. firstUncommittedSlot (nodeState' n) < i \<Longrightarrow> \<not> n \<midarrow>\<langle> PublishResponse i t \<rangle>\<leadsto>"
-        unfolding updated_properties apply (cases "n = n\<^sub>0", auto) done
-
-      from lastAcceptedTerm_None show "\<And>t. lastAcceptedTerm (nodeState' n) = None \<Longrightarrow> \<not> n \<midarrow>\<langle> PublishResponse (firstUncommittedSlot (nodeState' n)) t \<rangle>\<leadsto>"
-        unfolding updated_properties apply (cases "n = n\<^sub>0", auto simp add: firstUncommittedSlot_PublishResponse) done
-
-      from lastAcceptedTerm_Some_sent show "\<And>t. lastAcceptedTerm (nodeState' n) = Some t \<Longrightarrow> n \<midarrow>\<langle> PublishResponse (firstUncommittedSlot (nodeState' n)) t \<rangle>\<leadsto>"
-        unfolding updated_properties apply (cases "n = n\<^sub>0", auto) done
-
-      from lastAcceptedTerm_Some_max show "\<And>t t'. lastAcceptedTerm (nodeState' n) = Some t \<Longrightarrow> n \<midarrow>\<langle> PublishResponse (firstUncommittedSlot (nodeState' n)) t' \<rangle>\<leadsto> \<Longrightarrow> t' \<le> t"
-        unfolding updated_properties apply (cases "n = n\<^sub>0", auto) done
+      from lastAcceptedSlot_firstUncommittedSlot show "\<And>n. lastAcceptedSlot (nodeState n) \<le> firstUncommittedSlot (nodeState' n)"
+        unfolding updated_properties by auto
 
       from electionValueFree_JoinRequest show "\<And>n'. \<not> electionValueForced (nodeState' n) \<Longrightarrow> n' \<in> joinVotes (nodeState n) \<Longrightarrow> n' \<midarrow>\<langle> JoinRequest (firstUncommittedSlot (nodeState' n)) (currentTerm (nodeState n)) None \<rangle>\<rightarrow> (OneNode n) \<or> (\<exists>i<firstUncommittedSlot (nodeState' n). \<exists>a. n' \<midarrow>\<langle> JoinRequest i (currentTerm (nodeState n)) a \<rangle>\<rightarrow> (OneNode n))"
         unfolding updated_properties apply (cases "n = n\<^sub>0", auto)
         by (meson isMessageFromTo_def le_less_trans lessI zen.joinVotes zen_axioms)
 
-      from electionValueForced_JoinRequest show "electionValueForced (nodeState' n) \<Longrightarrow> \<not> (\<exists>x. \<langle> PublishRequest (firstUncommittedSlot (nodeState' n)) (currentTerm (nodeState n)) x \<rangle>\<leadsto>) \<Longrightarrow> \<exists>n'\<in>joinVotes (nodeState n). n' \<midarrow>\<langle> JoinRequest (firstUncommittedSlot (nodeState' n)) (currentTerm (nodeState n)) (lastAcceptedTerm (nodeState' n)) \<rangle>\<rightarrow> (OneNode n)"
+      from electionValueForced_JoinRequest show "electionValueForced (nodeState' n) \<Longrightarrow> \<not> (\<exists>x. \<langle> PublishRequest (firstUncommittedSlot (nodeState' n)) (currentTerm (nodeState n)) x \<rangle>\<leadsto>) \<Longrightarrow> \<exists>n'\<in>joinVotes (nodeState n). n' \<midarrow>\<langle> JoinRequest (firstUncommittedSlot (nodeState' n)) (currentTerm (nodeState n)) (lastAcceptedTermInSlot (nodeState' n)) \<rangle>\<rightarrow> (OneNode n)"
         unfolding updated_properties apply (cases "n = n\<^sub>0", auto) done
 
-      from electionValueForced_max show "\<And>n' a'. electionValueForced (nodeState' n) \<Longrightarrow> \<not> (\<exists>x. \<langle> PublishRequest (firstUncommittedSlot (nodeState' n)) (currentTerm (nodeState n)) x \<rangle>\<leadsto>) \<Longrightarrow> n' \<in> joinVotes (nodeState n) \<Longrightarrow> n' \<midarrow>\<langle> JoinRequest (firstUncommittedSlot (nodeState' n)) (currentTerm (nodeState n)) a' \<rangle>\<rightarrow> (OneNode n) \<Longrightarrow> maxTermOption a' (lastAcceptedTerm (nodeState' n)) = lastAcceptedTerm (nodeState' n)"
+      from electionValueForced_max show "\<And>n' a'. electionValueForced (nodeState' n) \<Longrightarrow> \<not> (\<exists>x. \<langle> PublishRequest (firstUncommittedSlot (nodeState' n)) (currentTerm (nodeState n)) x \<rangle>\<leadsto>) \<Longrightarrow> n' \<in> joinVotes (nodeState n) \<Longrightarrow> n' \<midarrow>\<langle> JoinRequest (firstUncommittedSlot (nodeState' n)) (currentTerm (nodeState n)) a' \<rangle>\<rightarrow> (OneNode n) \<Longrightarrow> maxTermOption a' (lastAcceptedTermInSlot (nodeState' n)) = lastAcceptedTermInSlot (nodeState' n)"
         unfolding updated_properties apply (cases "n = n\<^sub>0", auto) done
 
       from publishVotes show "\<And>n'. n' \<in> publishVotes (nodeState' n) \<Longrightarrow> n' \<midarrow>\<langle> PublishResponse (firstUncommittedSlot (nodeState' n)) (currentTerm (nodeState n)) \<rangle>\<leadsto>"
@@ -2431,17 +2490,11 @@ next
       from firstUncommittedSlot_PublishRequest show "\<And>i t x. firstUncommittedSlot (nodeState' n) < i \<Longrightarrow> \<not> n \<midarrow>\<langle> PublishRequest i t x \<rangle>\<leadsto>"
         unfolding updated_properties apply (cases "n = n\<^sub>0", auto) done
 
-      from lastAcceptedTerm_Some_value show "\<And>t. lastAcceptedTerm (nodeState' n) = Some t \<Longrightarrow> \<langle> PublishRequest (firstUncommittedSlot (nodeState' n)) t (lastAcceptedValue (nodeState' n)) \<rangle>\<leadsto>"
-        unfolding updated_properties apply (cases "n = n\<^sub>0", auto) done
-
       from PublishRequest_currentTerm show "\<And>t x. n \<midarrow>\<langle> PublishRequest (firstUncommittedSlot (nodeState' n)) t x \<rangle>\<leadsto> \<Longrightarrow> t \<le> currentTerm (nodeState n)"
         unfolding updated_properties apply (cases "n = n\<^sub>0", auto simp add: firstUncommittedSlot_PublishRequest) done
 
       from PublishRequest_publishPermitted_currentTerm show "\<And>t x. n \<midarrow>\<langle> PublishRequest (firstUncommittedSlot (nodeState' n)) t x \<rangle>\<leadsto> \<Longrightarrow> publishPermitted (nodeState' n) \<Longrightarrow> t < currentTerm (nodeState n)"
         unfolding updated_properties apply (cases "n = n\<^sub>0", auto simp add: firstUncommittedSlot_PublishRequest) done
-
-      from lastAcceptedTerm_Some_currentTerm show "\<And>t. lastAcceptedTerm (nodeState' n) = Some t \<Longrightarrow> t \<le> currentTerm (nodeState n)"
-        unfolding updated_properties apply (cases "n = n\<^sub>0", auto) done
 
       from currentClusterState_lastCommittedClusterStateBefore
       show "currentClusterState (nodeState' n) = lastCommittedClusterStateBefore (firstUncommittedSlot (nodeState' n))"
@@ -2480,6 +2533,9 @@ next
       "\<And>n. currentTerm (nodeState' n) = currentTerm (nodeState n)"
       "\<And>n. currentClusterState (nodeState' n) = currentClusterState (nodeState n)"
       "\<And>n. joinVotes (nodeState' n) = joinVotes (nodeState n)"
+      "\<And>n. lastAcceptedTerm (nodeState' n) = lastAcceptedTerm (nodeState n)"
+      "\<And>n. lastAcceptedValue (nodeState' n) = lastAcceptedValue (nodeState n)"
+      "\<And>n. lastAcceptedSlot (nodeState' n) = lastAcceptedSlot (nodeState n)"
       unfolding nodeState'_def by (auto simp add: nd' handleApplyCommit_def applyAcceptedValue_def nd_def)
 
     have updated_properties:
@@ -2487,14 +2543,16 @@ next
       "\<And>n. publishPermitted (nodeState' n) = (publishPermitted (nodeState n) \<or> n = n\<^sub>0)"
       "\<And>n. publishVotes (nodeState' n) = (if n = n\<^sub>0 then {} else publishVotes (nodeState n))"
       "\<And>n. electionValueForced (nodeState' n) = (electionValueForced (nodeState n) \<and> n \<noteq> n\<^sub>0)"
-      "\<And>n. lastAcceptedTerm (nodeState' n) = (if n = n\<^sub>0 then None else lastAcceptedTerm (nodeState n))"
-      "\<And>n. lastAcceptedValue (nodeState' n) = (if n = n\<^sub>0 then NoOp else lastAcceptedValue (nodeState n))"
       "\<And>n. currentVotingNodes (nodeState' n) = (if n = n\<^sub>0 then set newConfig else currentVotingNodes (nodeState n))"
       "\<And>n. electionWon (nodeState' n) = (if n = n\<^sub>0 then joinVotes nd \<in> majorities (set newConfig) else electionWon (nodeState n))"
       "\<And>n. isQuorum (nodeState' n) = (if n = n\<^sub>0 then (\<lambda>q. q \<in> majorities (set newConfig)) else isQuorum (nodeState n))"
       "\<And>n. currentVotingNodes (nodeState' n) = (if n = n\<^sub>0 then set newConfig else currentVotingNodes (nodeState n))"
       unfolding nodeState'_def using i t lastAcceptedValue_eq
       by (auto simp add: nd' handleApplyCommit_def applyAcceptedValue_def nd_def isQuorum_def)
+
+    have "\<And>n. lastAcceptedTermInSlot (nodeState' n) = (if n = n\<^sub>0 then None else lastAcceptedTermInSlot (nodeState n))"
+      unfolding lastAcceptedTermInSlot_def updated_properties property_simps by auto
+    note updated_properties = updated_properties this
 
     show ?thesis
       apply (intro zenI)
@@ -2520,6 +2578,11 @@ next
       from CatchUpResponse_committedTo show "\<And>i conf cs. \<langle> CatchUpResponse i conf cs \<rangle>\<leadsto> \<Longrightarrow> committed\<^sub>< i".
       from CatchUpResponse_V show "\<And>i conf cs. \<langle> CatchUpResponse i conf cs \<rangle>\<leadsto> \<Longrightarrow> V i = conf".
       from CatchUpResponse_lastCommittedClusterStateBefore show "\<And>i conf cs. \<langle> CatchUpResponse i conf cs \<rangle>\<leadsto> \<Longrightarrow> lastCommittedClusterStateBefore i = cs".
+      from lastAcceptedSlot_PublishResponse show "\<And>n i t. lastAcceptedSlot (nodeState n) < i \<Longrightarrow> \<not> n \<midarrow>\<langle> PublishResponse i t \<rangle>\<leadsto>".
+      from lastAcceptedTerm_None show "\<And>n t. lastAcceptedTerm (nodeState n) = None \<Longrightarrow> \<not> n \<midarrow>\<langle> PublishResponse (lastAcceptedSlot (nodeState n)) t \<rangle>\<leadsto>".
+      from lastAcceptedTerm_Some_sent show "\<And>n t. lastAcceptedTerm (nodeState n) = Some t \<Longrightarrow> n \<midarrow>\<langle> PublishResponse (lastAcceptedSlot (nodeState n)) t \<rangle>\<leadsto>".
+      from lastAcceptedTerm_Some_max show "\<And>n t t'. lastAcceptedTerm (nodeState n) = Some t \<Longrightarrow> n \<midarrow>\<langle> PublishResponse (lastAcceptedSlot (nodeState n)) t' \<rangle>\<leadsto> \<Longrightarrow> t' \<le> t".
+      from lastAcceptedTerm_Some_value show "\<And>n t. lastAcceptedTerm (nodeState n) = Some t \<Longrightarrow> \<langle> PublishRequest (lastAcceptedSlot (nodeState n)) t (lastAcceptedValue (nodeState n)) \<rangle>\<leadsto>".
 
       fix n
 
@@ -2527,17 +2590,8 @@ next
         unfolding updated_properties committedTo_def apply (cases "n = n\<^sub>0", auto)
         using i isCommitted_def less_antisym nd_def sent by blast
 
-      from firstUncommittedSlot_PublishResponse show "\<And>i t. firstUncommittedSlot (nodeState' n) < i \<Longrightarrow> \<not> n \<midarrow>\<langle> PublishResponse i t \<rangle>\<leadsto>"
-        unfolding updated_properties committedTo_def apply (cases "n = n\<^sub>0", auto) done
-
-      from lastAcceptedTerm_None show "\<And>t. lastAcceptedTerm (nodeState' n) = None \<Longrightarrow> \<not> n \<midarrow>\<langle> PublishResponse (firstUncommittedSlot (nodeState' n)) t \<rangle>\<leadsto>"
-        unfolding updated_properties apply (cases "n = n\<^sub>0", auto simp add: firstUncommittedSlot_PublishResponse) done
-
-      from lastAcceptedTerm_Some_sent show "\<And>t. lastAcceptedTerm (nodeState' n) = Some t \<Longrightarrow> n \<midarrow>\<langle> PublishResponse (firstUncommittedSlot (nodeState' n)) t \<rangle>\<leadsto>"
-        unfolding updated_properties apply (cases "n = n\<^sub>0", auto) done
-
-      from lastAcceptedTerm_Some_max show "\<And>t t'. lastAcceptedTerm (nodeState' n) = Some t \<Longrightarrow> n \<midarrow>\<langle> PublishResponse (firstUncommittedSlot (nodeState' n)) t' \<rangle>\<leadsto> \<Longrightarrow> t' \<le> t"
-        unfolding updated_properties apply (cases "n = n\<^sub>0", auto) done
+      from lastAcceptedSlot_firstUncommittedSlot show "\<And>n. lastAcceptedSlot (nodeState n) \<le> firstUncommittedSlot (nodeState' n)"
+        unfolding updated_properties by auto
 
       from electionWon_isQuorum show "\<And>n. electionWon (nodeState' n) \<Longrightarrow> isQuorum (nodeState' n) (joinVotes (nodeState n))"
         unfolding updated_properties apply (cases "n = n\<^sub>0", auto simp add: nd_def) done
@@ -2546,10 +2600,10 @@ next
         unfolding updated_properties apply (cases "n = n\<^sub>0", auto)
         by (meson isMessageFromTo_def le_imp_less_Suc zen.joinVotes zen_axioms)
 
-      from electionValueForced_JoinRequest show "electionValueForced (nodeState' n) \<Longrightarrow> \<not> (\<exists>x. \<langle> PublishRequest (firstUncommittedSlot (nodeState' n)) (currentTerm (nodeState n)) x \<rangle>\<leadsto>) \<Longrightarrow> \<exists>n'\<in>joinVotes (nodeState n). n' \<midarrow>\<langle> JoinRequest (firstUncommittedSlot (nodeState' n)) (currentTerm (nodeState n)) (lastAcceptedTerm (nodeState' n)) \<rangle>\<rightarrow> (OneNode n)"
+      from electionValueForced_JoinRequest show "electionValueForced (nodeState' n) \<Longrightarrow> \<not> (\<exists>x. \<langle> PublishRequest (firstUncommittedSlot (nodeState' n)) (currentTerm (nodeState n)) x \<rangle>\<leadsto>) \<Longrightarrow> \<exists>n'\<in>joinVotes (nodeState n). n' \<midarrow>\<langle> JoinRequest (firstUncommittedSlot (nodeState' n)) (currentTerm (nodeState n)) (lastAcceptedTermInSlot (nodeState' n)) \<rangle>\<rightarrow> (OneNode n)"
         unfolding updated_properties apply (cases "n = n\<^sub>0", auto) done
 
-      from electionValueForced_max show "\<And>n' a'. electionValueForced (nodeState' n) \<Longrightarrow> \<not> (\<exists>x. \<langle> PublishRequest (firstUncommittedSlot (nodeState' n)) (currentTerm (nodeState n)) x \<rangle>\<leadsto>) \<Longrightarrow> n' \<in> joinVotes (nodeState n) \<Longrightarrow> n' \<midarrow>\<langle> JoinRequest (firstUncommittedSlot (nodeState' n)) (currentTerm (nodeState n)) a' \<rangle>\<rightarrow> (OneNode n) \<Longrightarrow> maxTermOption a' (lastAcceptedTerm (nodeState' n)) = lastAcceptedTerm (nodeState' n)"
+      from electionValueForced_max show "\<And>n' a'. electionValueForced (nodeState' n) \<Longrightarrow> \<not> (\<exists>x. \<langle> PublishRequest (firstUncommittedSlot (nodeState' n)) (currentTerm (nodeState n)) x \<rangle>\<leadsto>) \<Longrightarrow> n' \<in> joinVotes (nodeState n) \<Longrightarrow> n' \<midarrow>\<langle> JoinRequest (firstUncommittedSlot (nodeState' n)) (currentTerm (nodeState n)) a' \<rangle>\<rightarrow> (OneNode n) \<Longrightarrow> maxTermOption a' (lastAcceptedTermInSlot (nodeState' n)) = lastAcceptedTermInSlot (nodeState' n)"
         unfolding updated_properties apply (cases "n = n\<^sub>0", auto) done
 
       from publishVotes show "\<And>n'. n' \<in> publishVotes (nodeState' n) \<Longrightarrow> n' \<midarrow>\<langle> PublishResponse (firstUncommittedSlot (nodeState' n)) (currentTerm (nodeState n)) \<rangle>\<leadsto>"
@@ -2565,9 +2619,6 @@ next
       from firstUncommittedSlot_PublishRequest show "\<And>i t x. firstUncommittedSlot (nodeState' n) < i \<Longrightarrow> \<not> n \<midarrow>\<langle> PublishRequest i t x \<rangle>\<leadsto>"
         unfolding updated_properties apply (cases "n = n\<^sub>0", auto) done
 
-      from lastAcceptedTerm_Some_value show "\<And>t. lastAcceptedTerm (nodeState' n) = Some t \<Longrightarrow> \<langle> PublishRequest (firstUncommittedSlot (nodeState' n)) t (lastAcceptedValue (nodeState' n)) \<rangle>\<leadsto>"
-        unfolding updated_properties apply (cases "n = n\<^sub>0", auto) done
-
       from PublishRequest_currentTerm show "\<And>t x. n \<midarrow>\<langle> PublishRequest (firstUncommittedSlot (nodeState' n)) t x \<rangle>\<leadsto> \<Longrightarrow> t \<le> currentTerm (nodeState n)"
         unfolding updated_properties apply (cases "n = n\<^sub>0", auto simp add: firstUncommittedSlot_PublishRequest) done
 
@@ -2581,7 +2632,7 @@ next
       from currentVotingNodes_firstUncommittedSlot show "\<And>n. currentVotingNodes (nodeState' n) = V (firstUncommittedSlot (nodeState' n))"
         unfolding updated_properties committedTo_def using Reconfigure i nd_def by (cases "n = n\<^sub>0", auto)
 
-      from lastAcceptedTerm_Some_currentTerm show "\<And>t. lastAcceptedTerm (nodeState' n) = Some t \<Longrightarrow> t \<le> currentTerm (nodeState n)"
+      from lastAcceptedTerm_Some_currentTerm show "\<And>t. lastAcceptedTerm (nodeState n) = Some t \<Longrightarrow> t \<le> currentTerm (nodeState n)"
         unfolding updated_properties apply (cases "n = n\<^sub>0", auto) done
     qed
   qed
@@ -2661,16 +2712,17 @@ proof -
     from JoinRequest_unique_destination show "\<And>i' i s t a a' d d'. s \<midarrow>\<langle> JoinRequest i t a \<rangle>\<rightarrow> d \<Longrightarrow> s \<midarrow>\<langle> JoinRequest i' t a' \<rangle>\<rightarrow> d' \<Longrightarrow> d = d'".
     from currentNode_nodeState show "\<And>n. currentNode (nodeState n) = n" .
     from committedTo_firstUncommittedSlot show "\<And>n. committed\<^sub>< (firstUncommittedSlot (nodeState n))" .
-    from firstUncommittedSlot_PublishResponse show "\<And>n i t. firstUncommittedSlot (nodeState n) < i \<Longrightarrow> \<not> n \<midarrow>\<langle> PublishResponse i t \<rangle>\<leadsto>" .
-    from lastAcceptedTerm_None show "\<And>n t. lastAcceptedTerm (nodeState n) = None \<Longrightarrow> \<not> n \<midarrow>\<langle> PublishResponse (firstUncommittedSlot (nodeState n)) t \<rangle>\<leadsto>".
-    from lastAcceptedTerm_Some_sent show "\<And>n t. lastAcceptedTerm (nodeState n) = Some t \<Longrightarrow> n \<midarrow>\<langle> PublishResponse (firstUncommittedSlot (nodeState n)) t \<rangle>\<leadsto>".
-    from lastAcceptedTerm_Some_max show "\<And>n t t'. lastAcceptedTerm (nodeState n) = Some t \<Longrightarrow> n \<midarrow>\<langle> PublishResponse (firstUncommittedSlot (nodeState n)) t' \<rangle>\<leadsto> \<Longrightarrow> t' \<le> t".
+    from lastAcceptedSlot_firstUncommittedSlot show "\<And>n. lastAcceptedSlot (nodeState n) \<le> firstUncommittedSlot (nodeState n)".
+    from lastAcceptedSlot_PublishResponse show "\<And>n i t. lastAcceptedSlot (nodeState n) < i \<Longrightarrow> \<not> n \<midarrow>\<langle> PublishResponse i t \<rangle>\<leadsto>" .
+    from lastAcceptedTerm_None show "\<And>n t. lastAcceptedTerm (nodeState n) = None \<Longrightarrow> \<not> n \<midarrow>\<langle> PublishResponse (lastAcceptedSlot (nodeState n)) t \<rangle>\<leadsto>".
+    from lastAcceptedTerm_Some_sent show "\<And>n t. lastAcceptedTerm (nodeState n) = Some t \<Longrightarrow> n \<midarrow>\<langle> PublishResponse (lastAcceptedSlot (nodeState n)) t \<rangle>\<leadsto>".
+    from lastAcceptedTerm_Some_max show "\<And>n t t'. lastAcceptedTerm (nodeState n) = Some t \<Longrightarrow> n \<midarrow>\<langle> PublishResponse (lastAcceptedSlot (nodeState n)) t' \<rangle>\<leadsto> \<Longrightarrow> t' \<le> t".
     from JoinRequest_currentTerm show "\<And>n i t a. n \<midarrow>\<langle> JoinRequest i t a \<rangle>\<leadsto> \<Longrightarrow> t \<le> currentTerm (nodeState n)".
     from JoinRequest_slot_function show "\<And>n i i' t a a'. n \<midarrow>\<langle> JoinRequest i t a \<rangle>\<leadsto> \<Longrightarrow> n \<midarrow>\<langle> JoinRequest i' t a' \<rangle>\<leadsto> \<Longrightarrow> i = i'".
     from electionWon_isQuorum show "\<And>n. electionWon (nodeState n) \<Longrightarrow> isQuorum (nodeState n) (joinVotes (nodeState n))".
     from electionValueFree_JoinRequest show "\<And>n n'. \<not> electionValueForced (nodeState n) \<Longrightarrow> n' \<in> joinVotes (nodeState n) \<Longrightarrow> n' \<midarrow>\<langle> JoinRequest (firstUncommittedSlot (nodeState n)) (currentTerm (nodeState n)) None \<rangle>\<rightarrow> (OneNode n) \<or> (\<exists>i<firstUncommittedSlot (nodeState n). \<exists>a. n' \<midarrow>\<langle> JoinRequest i (currentTerm (nodeState n)) a \<rangle>\<rightarrow> (OneNode n))".
-    from electionValueForced_JoinRequest show "\<And>n. electionValueForced (nodeState n) \<Longrightarrow> \<not> (\<exists>x. \<langle> PublishRequest (firstUncommittedSlot (nodeState n)) (currentTerm (nodeState n)) x \<rangle>\<leadsto>) \<Longrightarrow> \<exists>n'\<in>joinVotes (nodeState n). n' \<midarrow>\<langle> JoinRequest (firstUncommittedSlot (nodeState n)) (currentTerm (nodeState n)) (lastAcceptedTerm (nodeState n)) \<rangle>\<rightarrow> (OneNode n)".
-    from electionValueForced_max show " \<And>n n' a'. electionValueForced (nodeState n) \<Longrightarrow> \<not> (\<exists>x. \<langle> PublishRequest (firstUncommittedSlot (nodeState n)) (currentTerm (nodeState n)) x \<rangle>\<leadsto>) \<Longrightarrow> n' \<in> joinVotes (nodeState n) \<Longrightarrow> n' \<midarrow>\<langle> JoinRequest (firstUncommittedSlot (nodeState n)) (currentTerm (nodeState n)) a' \<rangle>\<rightarrow> (OneNode n) \<Longrightarrow> maxTermOption a' (lastAcceptedTerm (nodeState n)) = lastAcceptedTerm (nodeState n)".
+    from electionValueForced_JoinRequest show "\<And>n. electionValueForced (nodeState n) \<Longrightarrow> \<not> (\<exists>x. \<langle> PublishRequest (firstUncommittedSlot (nodeState n)) (currentTerm (nodeState n)) x \<rangle>\<leadsto>) \<Longrightarrow> \<exists>n'\<in>joinVotes (nodeState n). n' \<midarrow>\<langle> JoinRequest (firstUncommittedSlot (nodeState n)) (currentTerm (nodeState n)) (lastAcceptedTermInSlot (nodeState n)) \<rangle>\<rightarrow> (OneNode n)".
+    from electionValueForced_max show " \<And>n n' a'. electionValueForced (nodeState n) \<Longrightarrow> \<not> (\<exists>x. \<langle> PublishRequest (firstUncommittedSlot (nodeState n)) (currentTerm (nodeState n)) x \<rangle>\<leadsto>) \<Longrightarrow> n' \<in> joinVotes (nodeState n) \<Longrightarrow> n' \<midarrow>\<langle> JoinRequest (firstUncommittedSlot (nodeState n)) (currentTerm (nodeState n)) a' \<rangle>\<rightarrow> (OneNode n) \<Longrightarrow> maxTermOption a' (lastAcceptedTermInSlot (nodeState n)) = lastAcceptedTermInSlot (nodeState n)".
     from publishVotes show "\<And>n n'. n' \<in> publishVotes (nodeState n) \<Longrightarrow> n' \<midarrow>\<langle> PublishResponse (firstUncommittedSlot (nodeState n)) (currentTerm (nodeState n)) \<rangle>\<leadsto>".
     from publishVotes_currentVotingNodes show "\<And>n. publishVotes (nodeState n) \<subseteq> currentVotingNodes (nodeState n)".
     from currentClusterState_lastCommittedClusterStateBefore show "\<And>n. currentClusterState (nodeState n) = lastCommittedClusterStateBefore (firstUncommittedSlot (nodeState n))".
@@ -2682,7 +2734,7 @@ proof -
     from ApplyCommit_quorum show "\<And>i t. \<langle> ApplyCommit i t \<rangle>\<leadsto> \<Longrightarrow> \<exists>q\<in>majorities (V i). \<forall>s\<in>q. s \<midarrow>\<langle> PublishResponse i t \<rangle>\<leadsto>".
     from currentVotingNodes_firstUncommittedSlot show "\<And>n. currentVotingNodes (nodeState n) = V (firstUncommittedSlot (nodeState n))".
     from firstUncommittedSlot_PublishRequest show "\<And>i n t x. firstUncommittedSlot (nodeState n) < i \<Longrightarrow> \<not> n \<midarrow>\<langle> PublishRequest i t x \<rangle>\<leadsto>".
-    from lastAcceptedTerm_Some_value show "\<And>n t. lastAcceptedTerm (nodeState n) = Some t \<Longrightarrow> \<langle> PublishRequest (firstUncommittedSlot (nodeState n)) t (lastAcceptedValue (nodeState n)) \<rangle>\<leadsto>".
+    from lastAcceptedTerm_Some_value show "\<And>n t. lastAcceptedTerm (nodeState n) = Some t \<Longrightarrow> \<langle> PublishRequest (lastAcceptedSlot (nodeState n)) t (lastAcceptedValue (nodeState n)) \<rangle>\<leadsto>".
     from PublishRequest_currentTerm show "\<And>n t x. n \<midarrow>\<langle> PublishRequest (firstUncommittedSlot (nodeState n)) t x \<rangle>\<leadsto> \<Longrightarrow> t \<le> currentTerm (nodeState n)".
     from PublishRequest_publishPermitted_currentTerm show "\<And>n t x. n \<midarrow>\<langle> PublishRequest (firstUncommittedSlot (nodeState n)) t x \<rangle>\<leadsto> \<Longrightarrow> publishPermitted (nodeState n) \<Longrightarrow> t < currentTerm (nodeState n)".
     from lastAcceptedTerm_Some_currentTerm show "\<And>n t. lastAcceptedTerm (nodeState n) = Some t \<Longrightarrow> t \<le> currentTerm (nodeState n)".
@@ -2720,8 +2772,6 @@ next
   case True
 
   hence nd': "nd' = nd \<lparr> firstUncommittedSlot := i
-                , lastAcceptedValue := NoOp
-                , lastAcceptedTerm := None
                 , publishPermitted := False
                 , electionValueForced := False
                 , publishVotes := {}
@@ -2752,6 +2802,9 @@ next
   have property_simps[simp]:
     "\<And>n. currentNode (nodeState' n) = currentNode (nodeState n)"
     "\<And>n. currentTerm (nodeState' n) = currentTerm (nodeState n)"
+    "\<And>n. lastAcceptedTerm (nodeState' n) = lastAcceptedTerm (nodeState n)"
+    "\<And>n. lastAcceptedValue (nodeState' n) = lastAcceptedValue (nodeState n)"
+    "\<And>n. lastAcceptedSlot (nodeState' n) = lastAcceptedSlot (nodeState n)"
     unfolding nodeState'_def by (auto simp add: nd' nd_def)
 
   have updated_properties:
@@ -2759,8 +2812,6 @@ next
     "\<And>n. publishPermitted (nodeState' n) = (publishPermitted (nodeState n) \<and> n \<noteq> n\<^sub>0)"
     "\<And>n. publishVotes (nodeState' n) = (if n = n\<^sub>0 then {} else publishVotes (nodeState n))"
     "\<And>n. electionValueForced (nodeState' n) = (electionValueForced (nodeState n) \<and> n \<noteq> n\<^sub>0)"
-    "\<And>n. lastAcceptedTerm (nodeState' n) = (if n = n\<^sub>0 then None else lastAcceptedTerm (nodeState n))"
-    "\<And>n. lastAcceptedValue (nodeState' n) = (if n = n\<^sub>0 then NoOp else lastAcceptedValue (nodeState n))"
     "\<And>n. currentVotingNodes (nodeState' n) = (if n = n\<^sub>0 then conf else currentVotingNodes (nodeState n))"
     "\<And>n. joinVotes (nodeState' n) = (if n = n\<^sub>0 then {} else joinVotes (nodeState n))"
     "\<And>n. electionWon (nodeState' n) = (electionWon (nodeState n) \<and> n \<noteq> n\<^sub>0)"
@@ -2769,6 +2820,11 @@ next
     "\<And>n. currentClusterState (nodeState' n) = (if n = n\<^sub>0 then cs else currentClusterState (nodeState n))"
     unfolding nodeState'_def
     by (auto simp add: nd' nd_def isQuorum_def)
+
+  have "\<And>n. lastAcceptedTermInSlot (nodeState' n) = (if n = n\<^sub>0 then None else lastAcceptedTermInSlot (nodeState n))"
+    using True unfolding lastAcceptedTermInSlot_def updated_properties property_simps nd_def
+    using lastAcceptedSlot_firstUncommittedSlot not_le by auto
+  note updated_properties = updated_properties this
 
   show ?thesis
     apply (intro zenI)
@@ -2794,17 +2850,19 @@ next
     from CatchUpResponse_committedTo show "\<And>i conf cs. \<langle> CatchUpResponse i conf cs \<rangle>\<leadsto> \<Longrightarrow> committed\<^sub>< i".
     from CatchUpResponse_V show "\<And>i conf cs. \<langle> CatchUpResponse i conf cs \<rangle>\<leadsto> \<Longrightarrow> V i = conf".
     from CatchUpResponse_lastCommittedClusterStateBefore show "\<And>i conf cs. \<langle> CatchUpResponse i conf cs \<rangle>\<leadsto> \<Longrightarrow> lastCommittedClusterStateBefore i = cs".
+    from lastAcceptedTerm_None show "\<And>n t. lastAcceptedTerm (nodeState n) = None \<Longrightarrow> \<not> n \<midarrow>\<langle> PublishResponse (lastAcceptedSlot (nodeState n)) t \<rangle>\<leadsto>".
+    from lastAcceptedTerm_Some_sent show "\<And>n t. lastAcceptedTerm (nodeState n) = Some t \<Longrightarrow> n \<midarrow>\<langle> PublishResponse (lastAcceptedSlot (nodeState n)) t \<rangle>\<leadsto>".
+    from lastAcceptedSlot_PublishResponse show "\<And>n i t. lastAcceptedSlot (nodeState n) < i \<Longrightarrow> \<not> n \<midarrow>\<langle> PublishResponse i t \<rangle>\<leadsto>".
+    from lastAcceptedTerm_Some_max show "\<And>n t t'. lastAcceptedTerm (nodeState n) = Some t \<Longrightarrow> n \<midarrow>\<langle> PublishResponse (lastAcceptedSlot (nodeState n)) t' \<rangle>\<leadsto> \<Longrightarrow> t' \<le> t".
+    from lastAcceptedTerm_Some_value show "\<And>n t. lastAcceptedTerm (nodeState n) = Some t \<Longrightarrow> \<langle> PublishRequest (lastAcceptedSlot (nodeState n)) t (lastAcceptedValue (nodeState n)) \<rangle>\<leadsto>".
+    from lastAcceptedTerm_Some_currentTerm show "\<And>n t. lastAcceptedTerm (nodeState n) = Some t \<Longrightarrow> t \<le> currentTerm (nodeState n)".
+
+    from lastAcceptedSlot_firstUncommittedSlot show "\<And>n. lastAcceptedSlot (nodeState n) \<le> firstUncommittedSlot (nodeState' n)"
+      using True unfolding updated_properties nd_def using dual_order.strict_trans2 by fastforce
 
     from committedTo_firstUncommittedSlot show "\<And>n. committed\<^sub>< (firstUncommittedSlot (nodeState' n))"
       unfolding updated_properties apply auto
       using CatchUpResponse_committedTo sent by blast
-
-    from lastAcceptedTerm_None show "\<And>n t. lastAcceptedTerm (nodeState' n) = None \<Longrightarrow> \<not> n \<midarrow>\<langle> PublishResponse (firstUncommittedSlot (nodeState' n)) t \<rangle>\<leadsto>"
-      unfolding updated_properties apply auto
-      using True firstUncommittedSlot_PublishResponse nd_def by blast
-
-    from lastAcceptedTerm_Some_sent show "\<And>n t. lastAcceptedTerm (nodeState' n) = Some t \<Longrightarrow> n \<midarrow>\<langle> PublishResponse (firstUncommittedSlot (nodeState' n)) t \<rangle>\<leadsto>"
-      unfolding updated_properties apply auto done
 
     from electionWon_isQuorum show "\<And>n. electionWon (nodeState' n) \<Longrightarrow> isQuorum (nodeState' n) (joinVotes (nodeState' n))"
       unfolding updated_properties apply auto done
@@ -2812,10 +2870,10 @@ next
     from electionValueFree_JoinRequest show "\<And>n n'. \<not> electionValueForced (nodeState' n) \<Longrightarrow> n' \<in> joinVotes (nodeState' n) \<Longrightarrow> n' \<midarrow>\<langle> JoinRequest (firstUncommittedSlot (nodeState' n)) (currentTerm (nodeState n)) None \<rangle>\<rightarrow> (OneNode n) \<or> (\<exists>i<firstUncommittedSlot (nodeState' n). \<exists>a. n' \<midarrow>\<langle> JoinRequest i (currentTerm (nodeState n)) a \<rangle>\<rightarrow> (OneNode n))"
       unfolding updated_properties apply auto by blast
 
-    from electionValueForced_JoinRequest show "\<And>n. electionValueForced (nodeState' n) \<Longrightarrow> \<not> (\<exists>x. \<langle> PublishRequest (firstUncommittedSlot (nodeState' n)) (currentTerm (nodeState n)) x \<rangle>\<leadsto>) \<Longrightarrow> \<exists>n'\<in>joinVotes (nodeState' n). n' \<midarrow>\<langle> JoinRequest (firstUncommittedSlot (nodeState' n)) (currentTerm (nodeState n)) (lastAcceptedTerm (nodeState' n)) \<rangle>\<rightarrow> (OneNode n)"
+    from electionValueForced_JoinRequest show "\<And>n. electionValueForced (nodeState' n) \<Longrightarrow> \<not> (\<exists>x. \<langle> PublishRequest (firstUncommittedSlot (nodeState' n)) (currentTerm (nodeState n)) x \<rangle>\<leadsto>) \<Longrightarrow> \<exists>n'\<in>joinVotes (nodeState' n). n' \<midarrow>\<langle> JoinRequest (firstUncommittedSlot (nodeState' n)) (currentTerm (nodeState n)) (lastAcceptedTermInSlot (nodeState' n)) \<rangle>\<rightarrow> (OneNode n)"
       unfolding updated_properties apply auto done
 
-    from electionValueForced_max show " \<And>n n' a'. electionValueForced (nodeState' n) \<Longrightarrow> \<not> (\<exists>x. \<langle> PublishRequest (firstUncommittedSlot (nodeState' n)) (currentTerm (nodeState n)) x \<rangle>\<leadsto>) \<Longrightarrow> n' \<in> joinVotes (nodeState' n) \<Longrightarrow> n' \<midarrow>\<langle> JoinRequest (firstUncommittedSlot (nodeState' n)) (currentTerm (nodeState n)) a' \<rangle>\<rightarrow> (OneNode n) \<Longrightarrow> maxTermOption a' (lastAcceptedTerm (nodeState' n)) = lastAcceptedTerm (nodeState' n)"
+    from electionValueForced_max show " \<And>n n' a'. electionValueForced (nodeState' n) \<Longrightarrow> \<not> (\<exists>x. \<langle> PublishRequest (firstUncommittedSlot (nodeState' n)) (currentTerm (nodeState n)) x \<rangle>\<leadsto>) \<Longrightarrow> n' \<in> joinVotes (nodeState' n) \<Longrightarrow> n' \<midarrow>\<langle> JoinRequest (firstUncommittedSlot (nodeState' n)) (currentTerm (nodeState n)) a' \<rangle>\<rightarrow> (OneNode n) \<Longrightarrow> maxTermOption a' (lastAcceptedTermInSlot (nodeState' n)) = lastAcceptedTermInSlot (nodeState' n)"
       unfolding updated_properties apply auto done
 
     from publishVotes show "\<And>n n'. n' \<in> publishVotes (nodeState' n) \<Longrightarrow> n' \<midarrow>\<langle> PublishResponse (firstUncommittedSlot (nodeState' n)) (currentTerm (nodeState n)) \<rangle>\<leadsto>"
@@ -2829,18 +2887,8 @@ next
 
     fix n
 
-    from firstUncommittedSlot_PublishResponse show "\<And>i t. firstUncommittedSlot (nodeState' n) < i \<Longrightarrow> \<not> n \<midarrow>\<langle> PublishResponse i t \<rangle>\<leadsto>"
-      unfolding updated_properties apply (cases "n = n\<^sub>0", auto)
-      using True dual_order.strict_trans nd_def by blast
-
-    from lastAcceptedTerm_Some_max show "\<And>t t'. lastAcceptedTerm (nodeState' n) = Some t \<Longrightarrow> n \<midarrow>\<langle> PublishResponse (firstUncommittedSlot (nodeState' n)) t' \<rangle>\<leadsto> \<Longrightarrow> t' \<le> t"
-      unfolding updated_properties apply (cases "n = n\<^sub>0", auto) done
-
     from firstUncommittedSlot_PublishRequest show "\<And>i t x. firstUncommittedSlot (nodeState' n) < i \<Longrightarrow> \<not> n \<midarrow>\<langle> PublishRequest i t x \<rangle>\<leadsto>"
       unfolding updated_properties using True nd_def by (cases "n = n\<^sub>0", auto)
-
-    from lastAcceptedTerm_Some_value show "\<And>t. lastAcceptedTerm (nodeState' n) = Some t \<Longrightarrow> \<langle> PublishRequest (firstUncommittedSlot (nodeState' n)) t (lastAcceptedValue (nodeState' n)) \<rangle>\<leadsto>"
-      unfolding updated_properties apply (cases "n = n\<^sub>0", auto) done
 
     from PublishRequest_currentTerm show "\<And>t x. n \<midarrow>\<langle> PublishRequest (firstUncommittedSlot (nodeState' n)) t x \<rangle>\<leadsto> \<Longrightarrow> t \<le> currentTerm (nodeState n)"
       unfolding updated_properties apply (cases "n = n\<^sub>0", auto)
@@ -2855,9 +2903,6 @@ next
 
     from currentVotingNodes_firstUncommittedSlot show "\<And>n. currentVotingNodes (nodeState' n) = V (firstUncommittedSlot (nodeState' n))"
       unfolding updated_properties using CatchUpResponse_V sent by (cases "n = n\<^sub>0", auto)
-
-    from lastAcceptedTerm_Some_currentTerm show "\<And>t. lastAcceptedTerm (nodeState' n) = Some t \<Longrightarrow> t \<le> currentTerm (nodeState n)"
-      unfolding updated_properties apply (cases "n = n\<^sub>0", auto) done
   qed
 qed
 
@@ -2879,11 +2924,13 @@ proof -
     "\<And>n. firstUncommittedSlot (nodeState' n) = firstUncommittedSlot (nodeState n)"
     "\<And>n. currentVotingNodes (nodeState' n) = currentVotingNodes (nodeState n)"
     "\<And>n q. isQuorum (nodeState' n) q = isQuorum (nodeState n) q"
+    "\<And>n. lastAcceptedSlot (nodeState' n) = lastAcceptedSlot (nodeState n)"
     "\<And>n. lastAcceptedTerm (nodeState' n) = lastAcceptedTerm (nodeState n)"
     "\<And>n. lastAcceptedValue (nodeState' n) = lastAcceptedValue (nodeState n)"
+    "\<And>n. lastAcceptedTermInSlot (nodeState' n) = lastAcceptedTermInSlot (nodeState n)"
     "\<And>n. currentTerm (nodeState' n) = currentTerm (nodeState n)"
     "\<And>n. currentClusterState (nodeState' n) = currentClusterState (nodeState n)"
-    by (unfold nodeState'_def, auto simp add: nd_def isQuorum_def nd' handleReboot_def Let_def)
+    by (unfold nodeState'_def, auto simp add: nd_def isQuorum_def nd' handleReboot_def Let_def lastAcceptedTermInSlot_def)
 
   have updated_properties:
     "\<And>n. publishPermitted (nodeState' n) = (publishPermitted (nodeState n) \<and> n \<noteq> n\<^sub>0)"
@@ -2918,10 +2965,12 @@ proof -
     from JoinRequest_unique_destination show "\<And>i' i s t a a' d d'. s \<midarrow>\<langle> JoinRequest i t a \<rangle>\<rightarrow> d \<Longrightarrow> s \<midarrow>\<langle> JoinRequest i' t a' \<rangle>\<rightarrow> d' \<Longrightarrow> d = d'".
     from currentNode_nodeState show "\<And>n. currentNode (nodeState n) = n" .
     from committedTo_firstUncommittedSlot show "\<And>n. committed\<^sub>< (firstUncommittedSlot (nodeState n))" .
-    from firstUncommittedSlot_PublishResponse show "\<And>n i t. firstUncommittedSlot (nodeState n) < i \<Longrightarrow> \<not> n \<midarrow>\<langle> PublishResponse i t \<rangle>\<leadsto>" .
-    from lastAcceptedTerm_None show "\<And>n t. lastAcceptedTerm (nodeState n) = None \<Longrightarrow> \<not> n \<midarrow>\<langle> PublishResponse (firstUncommittedSlot (nodeState n)) t \<rangle>\<leadsto>".
-    from lastAcceptedTerm_Some_sent show "\<And>n t. lastAcceptedTerm (nodeState n) = Some t \<Longrightarrow> n \<midarrow>\<langle> PublishResponse (firstUncommittedSlot (nodeState n)) t \<rangle>\<leadsto>".
-    from lastAcceptedTerm_Some_max show "\<And>n t t'. lastAcceptedTerm (nodeState n) = Some t \<Longrightarrow> n \<midarrow>\<langle> PublishResponse (firstUncommittedSlot (nodeState n)) t' \<rangle>\<leadsto> \<Longrightarrow> t' \<le> t".
+    from lastAcceptedSlot_firstUncommittedSlot show "\<And>n. lastAcceptedSlot (nodeState n) \<le> firstUncommittedSlot (nodeState n)" .
+    from lastAcceptedSlot_PublishResponse show "\<And>n i t. lastAcceptedSlot (nodeState n) < i \<Longrightarrow> \<not> n \<midarrow>\<langle> PublishResponse i t \<rangle>\<leadsto>" .
+    from lastAcceptedTerm_None show "\<And>n t. lastAcceptedTerm (nodeState n) = None \<Longrightarrow> \<not> n \<midarrow>\<langle> PublishResponse (lastAcceptedSlot (nodeState n)) t \<rangle>\<leadsto>" .
+    from lastAcceptedTerm_Some_sent show "\<And>n t. lastAcceptedTerm (nodeState n) = Some t \<Longrightarrow> n \<midarrow>\<langle> PublishResponse (lastAcceptedSlot (nodeState n)) t \<rangle>\<leadsto>" .
+    from lastAcceptedTerm_Some_max show "\<And>n t t'. lastAcceptedTerm (nodeState n) = Some t \<Longrightarrow> n \<midarrow>\<langle> PublishResponse (lastAcceptedSlot (nodeState n)) t' \<rangle>\<leadsto> \<Longrightarrow> t' \<le> t" .
+    from lastAcceptedTerm_Some_value show "\<And>n t. lastAcceptedTerm (nodeState n) = Some t \<Longrightarrow> \<langle> PublishRequest (lastAcceptedSlot (nodeState n)) t (lastAcceptedValue (nodeState n)) \<rangle>\<leadsto>" .
     from JoinRequest_currentTerm show "\<And>n i t a. n \<midarrow>\<langle> JoinRequest i t a \<rangle>\<leadsto> \<Longrightarrow> t \<le> currentTerm (nodeState n)".
     from JoinRequest_slot_function show "\<And>n i i' t a a'. n \<midarrow>\<langle> JoinRequest i t a \<rangle>\<leadsto> \<Longrightarrow> n \<midarrow>\<langle> JoinRequest i' t a' \<rangle>\<leadsto> \<Longrightarrow> i = i'".
     from currentClusterState_lastCommittedClusterStateBefore show "\<And>n. currentClusterState (nodeState n) = lastCommittedClusterStateBefore (firstUncommittedSlot (nodeState n))".
@@ -2932,7 +2981,6 @@ proof -
     from ApplyCommit_quorum show "\<And>i t. \<langle> ApplyCommit i t \<rangle>\<leadsto> \<Longrightarrow> \<exists>q\<in>majorities (V i). \<forall>s\<in>q. s \<midarrow>\<langle> PublishResponse i t \<rangle>\<leadsto>".
     from currentVotingNodes_firstUncommittedSlot show "\<And>n. currentVotingNodes (nodeState n) = V (firstUncommittedSlot (nodeState n))".
     from firstUncommittedSlot_PublishRequest show "\<And>i n t x. firstUncommittedSlot (nodeState n) < i \<Longrightarrow> \<not> n \<midarrow>\<langle> PublishRequest i t x \<rangle>\<leadsto>".
-    from lastAcceptedTerm_Some_value show "\<And>n t. lastAcceptedTerm (nodeState n) = Some t \<Longrightarrow> \<langle> PublishRequest (firstUncommittedSlot (nodeState n)) t (lastAcceptedValue (nodeState n)) \<rangle>\<leadsto>".
     from PublishRequest_currentTerm show "\<And>n t x. n \<midarrow>\<langle> PublishRequest (firstUncommittedSlot (nodeState n)) t x \<rangle>\<leadsto> \<Longrightarrow> t \<le> currentTerm (nodeState n)".
     from CatchUpResponse_committedTo show "\<And>i conf cs. \<langle> CatchUpResponse i conf cs \<rangle>\<leadsto> \<Longrightarrow> committed\<^sub>< i".
     from CatchUpResponse_V show "\<And>i conf cs. \<langle> CatchUpResponse i conf cs \<rangle>\<leadsto> \<Longrightarrow> V i = conf".
@@ -2941,9 +2989,9 @@ proof -
 
     from electionWon_isQuorum show "\<And>n. electionWon (nodeState' n) \<Longrightarrow> isQuorum (nodeState n) (joinVotes (nodeState' n))"
       unfolding updated_properties by simp
-    from electionValueForced_JoinRequest show "\<And>n. electionValueForced (nodeState' n) \<Longrightarrow> \<not> (\<exists>x. \<langle> PublishRequest (firstUncommittedSlot (nodeState n)) (currentTerm (nodeState n)) x \<rangle>\<leadsto>) \<Longrightarrow> \<exists>n'\<in>joinVotes (nodeState' n). n' \<midarrow>\<langle> JoinRequest (firstUncommittedSlot (nodeState n)) (currentTerm (nodeState n)) (lastAcceptedTerm (nodeState n)) \<rangle>\<rightarrow> (OneNode n)"
+    from electionValueForced_JoinRequest show "\<And>n. electionValueForced (nodeState' n) \<Longrightarrow> \<not> (\<exists>x. \<langle> PublishRequest (firstUncommittedSlot (nodeState n)) (currentTerm (nodeState n)) x \<rangle>\<leadsto>) \<Longrightarrow> \<exists>n'\<in>joinVotes (nodeState' n). n' \<midarrow>\<langle> JoinRequest (firstUncommittedSlot (nodeState n)) (currentTerm (nodeState n)) (lastAcceptedTermInSlot (nodeState n)) \<rangle>\<rightarrow> (OneNode n)"
        unfolding updated_properties by simp
-    from electionValueForced_max show " \<And>n n' a'. electionValueForced (nodeState' n) \<Longrightarrow> \<not> (\<exists>x. \<langle> PublishRequest (firstUncommittedSlot (nodeState n)) (currentTerm (nodeState n)) x \<rangle>\<leadsto>) \<Longrightarrow> n' \<in> joinVotes (nodeState' n) \<Longrightarrow> n' \<midarrow>\<langle> JoinRequest (firstUncommittedSlot (nodeState n)) (currentTerm (nodeState n)) a' \<rangle>\<rightarrow> (OneNode n) \<Longrightarrow> maxTermOption a' (lastAcceptedTerm (nodeState n)) = lastAcceptedTerm (nodeState n)"
+    from electionValueForced_max show " \<And>n n' a'. electionValueForced (nodeState' n) \<Longrightarrow> \<not> (\<exists>x. \<langle> PublishRequest (firstUncommittedSlot (nodeState n)) (currentTerm (nodeState n)) x \<rangle>\<leadsto>) \<Longrightarrow> n' \<in> joinVotes (nodeState' n) \<Longrightarrow> n' \<midarrow>\<langle> JoinRequest (firstUncommittedSlot (nodeState n)) (currentTerm (nodeState n)) a' \<rangle>\<rightarrow> (OneNode n) \<Longrightarrow> maxTermOption a' (lastAcceptedTermInSlot (nodeState n)) = lastAcceptedTermInSlot (nodeState n)"
         unfolding updated_properties by simp
     from PublishRequest_publishPermitted_currentTerm show "\<And>n t x. n \<midarrow>\<langle> PublishRequest (firstUncommittedSlot (nodeState n)) t x \<rangle>\<leadsto> \<Longrightarrow> publishPermitted (nodeState' n) \<Longrightarrow> t < currentTerm (nodeState n)"
       unfolding updated_properties by simp
